Merge

concurrency/Cmm_op_proofs.thy
@@ -1,50 +1,125 @@
 theory Cmm_op_proofs
 
 imports
-  Main
-  "_bin/Cmm_op"
-  Cmm_master_lemmas
+Main
+"_bin/Cmm_op"
+Cmm_master_lemmas
+Nondeterminism_lemmas  
 begin
 
-(* The axiomatic model ------------------------------------------------- *)
+section {* The axiomatic model *}
 
 abbreviation "sublanguage \<equiv> true_condition"
 abbreviation "memory_model \<equiv> standard_memory_model"
 abbreviation "axBehaviour \<equiv> standard_behaviour"
 abbreviation "axUndefined \<equiv> locks_only_undefined_behaviour_alt"
 abbreviation "getRelations \<equiv> standard_relations"
+abbreviation "getHb \<equiv> with_consume_hb"
+abbreviation "getVse \<equiv> with_consume_vse"
 abbreviation "axConsistent ex \<equiv> apply_tree standard_consistent_execution ex"
+abbreviation "axConsistentAlt pre wit \<equiv> axConsistent (pre, wit, getRelations pre wit)"
 
 lemmas sublanguage_def = true_condition_def
 lemmas memory_model_def = with_consume_memory_model_def
 lemmas axBehaviour_def = standard_behaviour_def
 lemmas axUndefined_def = locks_only_undefined_behaviour_alt_def
 lemmas getRelations_def = standard_relations_def
+lemmas getHb_def = with_consume_hb_def
+lemmas getVse_def = with_consume_vse_def
 lemmas axConsistent_def = standard_consistent_execution_def
+lemmas axConsistentAlt_def = axConsistent_def
 
 lemmas getRelations_simp = standard_relations_simp
                            standard_relations_alt_def
 
 
 
-(* The simplified axiomatic model ------------------------------------- *)
+section {* The simplified axiomatic model *}
 
 abbreviation "axsimpConsistent ex \<equiv> apply_tree axsimpConsistentExecution ex"
+abbreviation "axsimpConsistentAlt pre wit \<equiv> axsimpConsistent (pre, wit, getRelations pre wit)"
 
 lemmas axsimpConsistent_def = axsimpConsistentExecution_def
+lemmas axsimpConsistentAlt_def = axsimpConsistent_def
+
+lemma rel_list_well_formed_threads_opsem [simp]:
+  assumes "rel \<noteq> []"
+  shows   "well_formed_threads_opsem (pre, wit, rel) = well_formed_threads_opsem (pre, wit, [])"
+using assms
+unfolding well_formed_threads_opsem.simps
+by simp
+
+lemma witness_well_formed_threads_opsem [simp]:
+  assumes "wit \<noteq> empty_witness"
+  shows   "well_formed_threads_opsem (pre, wit, []) = well_formed_threads_opsem (pre, empty_witness, [])"
+using assms
+unfolding well_formed_threads_opsem.simps
+by simp
+
+lemma well_formed_threads_opsem_eq:
+  shows "  well_formed_threads_opsem (pre, wit, rel)
+         = (well_formed_threads (pre, wit, rel) \<and> finite (actions0 pre))"
+unfolding well_formed_threads_opsem.simps
+..
+
+lemma  well_formed_threads_opsemE [elim]:
+  assumes "well_formed_threads_opsem (pre, wit, rel)"
+  obtains "finite (actions0 pre)"
+      and "actions_respect_location_kinds (actions0 pre) (lk pre)"  
+      and "blocking_observed (actions0 pre) (sb pre)"  
+      and "inj_on aid_of (actions0 pre)"  
+      and "relation_over (actions0 pre) (sb pre)"  
+      and "relation_over (actions0 pre) (asw pre) "  
+      and "threadwise (actions0 pre) (sb pre)"  
+      and "interthread (actions0 pre) (asw pre)"  
+      and "isStrictPartialOrder (sb pre)"  
+      and "isStrictPartialOrder (dd pre)"  
+      and "(dd pre) \<subseteq> (sb pre)"  
+      and "indeterminate_sequencing pre"  
+      and "irrefl (sbasw pre)"  
+      and "finite_prefixes (sbasw pre) (actions0 pre)"  
+      and "disjoint_allocs (actions0 pre)"
+using assms
+unfolding well_formed_threads_opsem_eq
+by auto
+
+lemma axsimpConsistentE [elim]: 
+  assumes "axsimpConsistentAlt pre wit"
+  obtains "assumptions (pre, wit, [])"
+      and "tot_empty (pre, wit, [])"
+      and "well_formed_threads_opsem (pre, wit, [])"
+      and "well_formed_rf (pre, wit, [])"
+      and "locks_only_consistent_locks (pre, wit, [])"
+      and "locks_only_consistent_lo (pre, wit, [(''hb'', getHb pre wit)])"
+      and "consistent_mo (pre, wit, [])"
+      and "sc_accesses_consistent_sc (pre, wit, [(''hb'', getHb pre wit)])"
+      and "sc_fenced_sc_fences_heeded (pre, wit, [])"
+      and "consistent_hb (pre, wit, [(''hb'', getHb pre wit)])"
+      and "det_read_alt (pre, wit, [(''hb'', getHb pre wit)])"
+      and "consistent_non_atomic_rf (pre, wit, [(''hb'', getHb pre wit), 
+                                                (''vse'', getVse pre wit)])"
+      and "consistent_atomic_rf (pre, wit, [(''hb'', getHb pre wit)])"
+      and "coherent_memory_use (pre, wit, [(''hb'', getHb pre wit)])"
+      and "rmw_atomicity (pre, wit, [])"
+      and "sc_accesses_sc_reads_restricted (pre, wit, [(''hb'', getHb pre wit)])"
+using assms
+unfolding axsimpConsistent_def
+          memory_model_def
+by simp_all
 
 lemma axsimpConsistentEq:
   fixes pre wit
   defines "ex \<equiv> (pre, wit, getRelations pre wit)"
-  shows   "axsimpConsistent ex = axConsistent ex"
-using assms
-      det_read_simp 
+  shows   "axsimpConsistent ex = (axConsistent ex \<and> finite (actions0 pre))"
+using det_read_simp 
       standard_consistent_atomic_rf_simp
-unfolding axsimpConsistent_def
+      well_formed_threads_opsem_eq
+unfolding axsimpConsistent_def 
           axConsistent_def
           getRelations_simp 
           with_consume_vse_def
-by auto
+          ex_def 
+by simp metis
 
 lemma axsimpMemoryModel_simps [simp]:
   shows "consistent axsimpMemoryModel = axsimpConsistentExecution"
@@ -53,7 +128,9 @@ lemma axsimpMemoryModel_simps [simp]:
 unfolding axsimpMemoryModel_def
 by simp_all
 
-lemma axBehaviourEq:
+(* Not true anymore. *)
+(*
+lemma axsimpBehaviourEq:
   shows "axsimpBehaviour = axBehaviour"
 proof (intro ext)
   fix opsem_t
@@ -66,10 +143,3157 @@ proof (intro ext)
     unfolding axsimpBehaviour_def axBehaviour_def
               behaviour_def Let_def
     by simp
+qed *)
+
+section {* The incremental model *}
+
+abbreviation "hbMinusAlt pre wit \<equiv> hbMinus (pre,wit, getRelations pre wit)"
+abbreviation "incComAlt pre wit \<equiv> incCom (pre,wit, getRelations pre wit)"
+
+lemmas hbMinusAlt_def = hbMinus.simps
+lemmas incComAlt_def = incCom.simps
+
+subsection {* Simplifications *}
+
+lemma incPreRestrict_simps [simp]:
+  shows "actions0 (preRestrict pre actions) = actions0 pre \<inter> actions "
+        "threads (preRestrict pre actions) = threads pre"
+        "lk (preRestrict pre actions) = lk pre"
+        "sb (preRestrict pre actions) = relRestrict (sb pre) actions"
+        "asw (preRestrict pre actions) = relRestrict (asw pre) actions"
+        "dd (preRestrict pre actions) = relRestrict (dd pre) actions"
+unfolding preRestrict_def
+by simp_all
+
+lemma preRestrict_id:
+  assumes "well_formed_threads_opsem (pre, empty_witness, [])"
+  shows   "preRestrict pre (actions0 pre) = pre"
+proof -
+  have sb: "relOver (sb pre) (actions0 pre)"
+    using assms by auto
+  have asw: "relOver (asw pre) (actions0 pre)"
+    using assms by auto
+  have "dd pre \<subseteq> sb pre"
+    using assms by auto
+  hence dd: "relOver (dd pre) (actions0 pre)"
+    using sb relOver_subset by metis
+  show ?thesis
+    using relRestrict_id[OF sb] 
+          relRestrict_id[OF dd] 
+          relRestrict_id[OF asw]
+    unfolding preRestrict_def
+    by simp
+qed
+
+lemma incPreRestrict_sbasw_empty [simp]:
+  shows "sbasw (preRestrict pre {}) = {}"
+unfolding sbasw_def
+by simp
+
+lemma incPreRestrict_sbasw_subset:
+  shows "sbasw (preRestrict pre actions) \<subseteq> relRestrict (sbasw pre) actions"
+proof -
+  have "sbasw (preRestrict pre actions) = (relRestrict (sb pre \<union> asw pre) actions)\<^sup>+"
+    unfolding sbasw_def by simp
+  also have "... \<subseteq> relRestrict (sbasw pre) actions"
+    unfolding sbasw_def
+    using relRestrict_trancl_subset
+    by metis
+  finally show ?thesis .
+qed
+
+lemma incPreRestrict_sbasw_subset2:
+  shows "sbasw (preRestrict pre actions) \<subseteq> sbasw pre"
+using incPreRestrict_sbasw_subset
+unfolding relRestrict_def
+by auto
+
+lemma incWitRestrict_simps [simp]:
+  shows "rf (incWitRestrict wit actions) = relRestrict (rf wit) actions"
+        "mo (incWitRestrict wit actions) = relRestrict (mo wit) actions"
+        "sc (incWitRestrict wit actions) = relRestrict (sc wit) actions"
+        "lo (incWitRestrict wit actions) = relRestrict (lo wit) actions"
+        "tot (incWitRestrict wit actions) = relRestrict (tot wit) actions"
+unfolding incWitRestrict_def
+by simp_all
+
+lemma incWitRestrict_empty1 [simp]:
+  shows "incWitRestrict wit {} = empty_witness"
+unfolding incWitRestrict_def empty_witness_def 
+by simp
+
+lemma incWitRestrict_empty2 [simp]:
+  shows "incWitRestrict empty_witness x = empty_witness"
+unfolding incWitRestrict_def empty_witness_def 
+by simp
+
+lemma incWitRestrict_multiple [simp]:
+  shows "incWitRestrict (incWitRestrict x y) z = incWitRestrict x (y \<inter> z)"
+unfolding incWitRestrict_def 
+by auto
+
+lemma initialState_simps [simp]:
+  shows "incWit (incInitialState pre) = empty_witness"
+        "incCommitted (incInitialState pre) = {}"
+unfolding incInitialState_def
+by simp_all
+
+lemma hbMinusE [elim]:
+  assumes "(a, b) \<in> hbMinus (pre, wit, (''hb'', hb)#rel)"
+  obtains "(a, b) \<in> hb"
+      and "is_na_or_non_write pre b"
+using assms
+unfolding hbMinus.simps
+by auto
+
+lemma hbMinus_relation_rel_list [simp]:
+  assumes "rel \<noteq> []"
+  shows "  hbMinus (pre, wit, (''hb'', hb)#rel) 
+         = hbMinus (pre, wit, [(''hb'', hb)])"
+unfolding hbMinus.simps ..
+
+lemma hbMinus_relation_rel_list2 [simp]:
+  shows "  hbMinus (pre, wit, getRelations pre wit) 
+         = hbMinus (pre, wit, [(''hb'', getHb pre wit)])"
+unfolding getRelations_simp by simp
+
+lemma is_na_or_non_write_relRestrict_simp [simp]:
+  shows "  is_na_or_non_write (preRestrict pre actions) b
+         = is_na_or_non_write pre b"
+unfolding is_na_or_non_write_def
+by auto
+
+subsection {* Commitment order *}
+
+lemma not_at_writes_in_hb_minus:
+  assumes cons:         "axsimpConsistentAlt pre wit"
+      and in_rel:       "(a, b) \<in> hbMinusAlt pre wit \<union> rf wit \<union> mo wit"
+      and not_at_write: "is_na_or_non_write pre a"
+  shows                 "(a, b) \<in> hbMinusAlt pre wit"
+using in_rel
+proof (elim UnE)
+  assume in_rf: "(a, b) \<in> rf wit"
+  hence "is_write a" "is_read b" "loc_of a = loc_of b" 
+    using cons by auto
+  hence "is_at_non_atomic_location (lk pre) a"
+    using not_at_write unfolding is_na_or_non_write_def by simp
+  hence not_at: "is_at_non_atomic_location (lk pre) b"
+    using `loc_of a = loc_of b` 
+    unfolding is_at_non_atomic_location_def by auto
+  hence "(a, b) \<in> getVse pre wit"
+    using in_rf cons by auto
+  hence in_hb: "(a, b) \<in> getHb pre wit"
+    by auto
+  have "is_na_or_non_write pre b"
+    using not_at unfolding is_na_or_non_write_def by simp
+  thus "(a, b) \<in> hbMinusAlt pre wit"
+    using in_hb
+    (* TODO: fix how hbMinus works, so we don't have to do simp before unfolding. *)
+    apply simp
+    unfolding hbMinusAlt_def
+    by auto
+next
+  assume "(a, b) \<in> mo wit"
+  hence "is_write a \<and> is_at_atomic_location (lk pre) a"
+    using cons by auto
+  hence False
+    using not_at_write 
+    unfolding is_na_or_non_write_def
+    by auto
+  thus "(a, b) \<in> hbMinusAlt pre wit" 
+    by contradiction auto
+qed auto
+
+lemma not_at_writes_in_hb_minus_tc:
+  assumes cons:         "axsimpConsistent (pre, wit, getRelations pre wit)"
+      and in_tc_rel:    "(a, b) \<in> (hbMinusAlt pre wit \<union> rf wit \<union> mo wit)\<^sup>+"
+      and not_at_write: "is_na_or_non_write pre a"
+  shows                 "(a, b) \<in> (hbMinusAlt pre wit)\<^sup>+" 
+proof (rule trancl_induct[OF in_tc_rel])
+  fix y
+  assume in_rel: "(a, y) \<in> hbMinusAlt pre wit \<union> rf wit \<union> mo wit"
+  have "(a, y) \<in> hbMinusAlt pre wit" 
+    using not_at_writes_in_hb_minus[OF cons in_rel not_at_write] .
+  thus "(a, y) \<in> (hbMinusAlt pre wit)\<^sup>+" by auto
+next
+  fix y z
+  assume ay_in_rel: "(a, y) \<in> (hbMinusAlt pre wit \<union> rf wit \<union> mo wit)\<^sup>+"
+     and yz_in_rel: "(y, z) \<in> hbMinusAlt pre wit \<union> rf wit \<union> mo wit"
+     and ay_in_tc:  "(a, y) \<in> (hbMinusAlt pre wit)\<^sup>+"
+  hence "\<exists>c. (c, y) \<in> hbMinusAlt pre wit" 
+    using tranclD2[where R="(hbMinusAlt pre wit)"] by auto
+  hence "is_na_or_non_write pre y" by auto
+  hence "(y, z) \<in> hbMinusAlt pre wit"
+    using not_at_writes_in_hb_minus[OF cons yz_in_rel] by auto
+  thus "(a, z) \<in> (hbMinusAlt pre wit)\<^sup>+" 
+    using ay_in_tc by (auto simp add: trancl_into_trancl)
+qed
+
+lemma at_writes_in_mo:
+  assumes cons:        "axsimpConsistent (pre, wit, getRelations pre wit)"
+      and in_rel:      "(a, b) \<in> hbMinusAlt pre wit \<union> rf wit \<union> mo wit"
+      and is_at_write: "\<not>is_na_or_non_write pre b"
+  shows                "(a, b) \<in> mo wit"
+using in_rel
+proof (elim UnE)
+  assume "(a, b) \<in> hbMinusAlt pre wit"
+  hence "is_na_or_non_write pre b" by auto
+  hence False using is_at_write by simp
+  thus ?thesis by simp
+next
+  assume in_rf: "(a, b) \<in> rf wit"
+  hence "is_read b" using cons by auto
+  hence "is_RMW b" 
+    using is_at_write
+    unfolding is_na_or_non_write_def
+    by (cases b) simp_all
+  thus "(a, b) \<in> mo wit"
+    using in_rf cons by auto
+qed auto
+
+lemma at_writes_in_mo_tc:
+  assumes cons:        "axsimpConsistent (pre, wit, getRelations pre wit)"
+      and in_rel_tc:   "(a, b) \<in> (hbMinusAlt pre wit \<union> rf wit \<union> mo wit)\<^sup>+"
+      and is_at_write: "\<not>is_na_or_non_write pre b"
+  shows                "(a, b) \<in> (mo wit)\<^sup>+"
+proof (rule converse_trancl_induct[OF in_rel_tc]) 
+  fix y
+  assume in_rel: "(y, b) \<in> hbMinusAlt pre wit \<union> rf wit \<union> mo wit"
+  have "(y, b) \<in> mo wit" using at_writes_in_mo[OF cons in_rel is_at_write] .
+  thus "(y, b) \<in> (mo wit)\<^sup>+" by auto
+next
+  fix y z
+  assume "(y, z) \<in> hbMinusAlt pre wit \<union> rf wit \<union> mo wit"
+         "(z, b) \<in> (hbMinusAlt pre wit \<union> rf wit \<union> mo wit)\<^sup>+"
+         "(z, b) \<in> (mo wit)\<^sup>+"
+  hence "\<exists>c. (z, c) \<in> mo wit" 
+    using tranclD[where R="mo wit"] by auto
+  hence "is_write z" "is_at_atomic_location (lk pre) z"
+    using cons by auto
+  hence "\<not> is_na_or_non_write pre z" 
+    unfolding is_na_or_non_write_def
+    by auto
+  hence "(y, z) \<in> mo wit"
+    using `(y, z) \<in> hbMinusAlt pre wit \<union> rf wit \<union> mo wit`
+    using at_writes_in_mo[OF cons] by auto
+  thus "(y, b) \<in> (mo wit)\<^sup>+" 
+    using `(z, b) \<in> (mo wit)\<^sup>+` 
+    by (auto simp add: trancl_into_trancl)
+qed 
+
+lemma opsemOrder_isStrictPartialOrder:
+  assumes cons: "axsimpConsistent (pre, wit, getRelations pre wit)"
+  shows         "isStrictPartialOrder (incComAlt pre wit)"
+proof -
+  have "irrefl (incComAlt pre wit)"
+    unfolding irrefl_def
+    proof (intro allI notI)
+      fix x
+      assume "(x, x) \<in> incComAlt pre wit"
+      hence in_rel: "(x, x) \<in> (hbMinusAlt pre wit \<union> rf wit \<union> mo wit)\<^sup>+"
+        unfolding incComAlt_def
+        by (metis Un_assoc)
+      show False
+        proof (cases "is_na_or_non_write pre x")
+          have cons_hb: "consistent_hb (pre, wit, [(''hb'', getHb pre wit)])"
+            using cons by auto
+          have "(hbMinusAlt pre wit) \<subseteq> getHb pre wit" by auto
+          hence hbMinus_in_hb: "(hbMinusAlt pre wit)\<^sup>+ \<subseteq> (getHb pre wit)\<^sup>+" 
+            using trancl_mono by auto
+          hence irrefl_hbMinus: "irrefl ((hbMinusAlt pre wit)\<^sup>+)"
+            using cons_hb
+            unfolding consistent_hb.simps irrefl_def
+            by auto
+          assume "is_na_or_non_write pre x"
+          hence "(x, x) \<in> (hbMinusAlt pre wit)\<^sup>+" 
+            using not_at_writes_in_hb_minus_tc[OF cons in_rel] by metis
+          thus False using irrefl_hbMinus unfolding irrefl_def by metis         
+        next
+          have cons_mo: "consistent_mo (pre, wit, [])"
+            using cons by auto
+          assume "\<not>is_na_or_non_write pre x"
+          hence "(x, x) \<in> (mo wit)\<^sup>+" 
+            using at_writes_in_mo_tc[OF cons in_rel] by metis
+          hence "(x, x) \<in> mo wit"
+            using cons_mo unfolding consistent_mo.simps by simp
+          thus False
+            using cons_mo unfolding consistent_mo.simps irrefl_def by simp            
+        qed
+    qed
+  thus "isStrictPartialOrder (incComAlt pre wit)" 
+    unfolding isStrictPartialOrder_def incComAlt_def by simp
+qed
+
+(* We define a specialised induction rule for downclosed finite sets. *)
+lemma finite_downclosedsubset_induct:
+  assumes fin:        "finite A"
+      and universe:   "A \<subseteq> B"
+      and downclosed: "downclosed A R"
+      and order:      "acyclic R"
+      and empty:      "P {}"
+      and step:       "\<And>a F. finite F \<Longrightarrow> 
+                          a \<in> B \<Longrightarrow> 
+                          a \<notin> F \<Longrightarrow> 
+                          (\<forall>b\<in>F. (a, b) \<notin> R) \<Longrightarrow> 
+                          P F \<Longrightarrow> 
+                          downclosed (insert a F) R \<Longrightarrow> 
+                          P (insert a F)"
+  shows           "P A"
+using fin empty downclosed universe
+proof (induct rule: finite_psubset_induct)
+  fix A
+  assume fin:        "finite A"
+     and IH:         "\<And>C. C \<subset> A \<Longrightarrow> P {} \<Longrightarrow> downclosed C R \<Longrightarrow> C \<subseteq> B \<Longrightarrow> P C"
+     and empty:      "P {}"
+     and downclosed: "downclosed A R"
+     and universe:   "A \<subseteq> B"
+  show "P A"
+    proof (cases "A = {}")
+      assume "A = {}"
+      thus "P A" using empty by metis
+    next
+      assume "A \<noteq> {}"
+      obtain x where sup: "x \<in> A \<and> (\<forall>y. (x, y) \<in> R \<longrightarrow> y \<notin> A)"
+        using fin `A \<noteq> {}` order by (metis supremum)
+      have "x \<in> B" using universe sup by auto
+      let ?F = "A - {x}"
+      have insert: "x \<notin> ?F" "A = insert x ?F" "?F \<subset> A" using sup by auto
+      have downclosed_f: "downclosed ?F R"
+        using downclosed sup unfolding downclosed_def by auto
+      have downclosed_insert_f: "downclosed (insert x ?F) R"
+        using downclosed insert by auto
+      have finite_f: "finite ?F" using fin insert by auto
+      have universe_f: "?F \<subseteq> B" using universe by auto
+      have "P ?F" using IH[OF `?F \<subset> A` empty downclosed_f universe_f] .
+      have max: "\<forall>b\<in>?F. (x, b) \<notin> R" using sup by auto
+      show "P A" 
+        using step[OF finite_f `x \<in> B` `x \<notin> ?F` max `P ?F` downclosed_insert_f] 
+        using `A = insert x ?F` 
+        by simp
+   qed
+qed
+
+subsection {* Properties of happens-before *}
+
+subsubsection {* RelOver *}
+
+(* In this section we prove all properties of getHb that we need, so after this section we never
+   need to unfold the definition of hb. This way, if hb changes, we only need to change this 
+   section. *)
+
+(* RelOver in the rel-acq-rlx fragment *)
+
+lemma relOver_release_acquire_relaxed_sw:
+  shows   "relOver (release_acquire_relaxed_synchronizes_with_set_alt pre wit) (actions0 pre)"
+unfolding release_acquire_relaxed_synchronizes_with_set_alt_def
+          release_acquire_relaxed_synchronizes_with_set_def 
+unfolding relOver_def 
+by auto
+ 
+lemma relOver_release_acquire_relaxed_hb:
+  assumes "relOver (sb pre) (actions0 pre)"
+  shows   "relOver (release_acquire_relaxed_hb pre wit) (actions0 pre)"
+unfolding release_acquire_relaxed_hb_def no_consume_hb_def
+using assms relOver_release_acquire_relaxed_sw
+by simp
+
+(* RelOver in the rel-acq-rlx-fence fragment *)
+
+lemma relOver_release_acquire_fenced_sw:
+  shows   "relOver (release_acquire_fenced_synchronizes_with_set_alt pre wit) (actions0 pre) "
+unfolding release_acquire_fenced_synchronizes_with_set_alt_def
+          release_acquire_fenced_synchronizes_with_set_def 
+unfolding relOver_def 
+(* TODO define relOver elim for all the relations *)
+unfolding sw_asw_def
+          sw_lock_def
+          sw_rel_acq_rs_def
+          sw_fence_sb_hrs_rf_sb_def
+          sw_fence_sb_hrs_rf_def
+          sw_fence_rs_rf_sb_def
+by auto
+ 
+lemma relOver_release_acquire_fenced_hb:
+  assumes "relOver (sb pre) (actions0 pre)"
+  shows   "relOver (release_acquire_fenced_hb pre wit) (actions0 pre)"
+unfolding release_acquire_fenced_hb_def no_consume_hb_def
+using assms relOver_release_acquire_fenced_sw
+by simp
+
+(* RelOver in the with_consume fragment *)
+
+lemma relOver_dob:
+  shows   "relOver (with_consume_dob_set_alt pre wit) (actions0 pre)"
+unfolding with_consume_dob_set_alt_def with_consume_dob_set_def 
+unfolding relOver_def 
+by auto
+
+lemma relOver_ithb:
+  assumes "relOver (sb pre) (actions0 pre)"
+  shows   "relOver (inter_thread_happens_before_alt pre wit) (actions0 pre)"
+unfolding inter_thread_happens_before_alt_def
+          inter_thread_happens_before_step_def
+          inter_thread_happens_before_r_def
+using assms relOver_dob relOver_release_acquire_fenced_sw
+by (simp add: relOver_relComp)
+ 
+lemma relOver_with_consume_hb:
+  assumes "relOver (sb pre) (actions0 pre)"
+  shows   "relOver (with_consume_hb pre wit) (actions0 pre)"
+unfolding with_consume_hb_def happens_before_def
+using assms relOver_ithb
+by simp
+
+subsubsection {* Empty hb *}
+
+(* Empty hb in the with_consume fragment *)
+
+lemma sw_asw_empty [simp]:
+  shows "sw_asw (preRestrict pre {}) empty_witness = {}"
+unfolding sw_asw_def
+by simp
+
+lemma sw_lock_empty [simp]:
+  shows "sw_lock (preRestrict pre {}) empty_witness = {}"
+unfolding sw_lock_def
+by simp
+
+lemma sw_rel_acq_rs_empty [simp]:
+  shows "sw_rel_acq_rs (preRestrict pre {}) empty_witness = {}"
+unfolding sw_rel_acq_rs_def
+by simp
+
+lemma sw_fence_sb_hrs_rf_sb_empty [simp]:
+  shows "sw_fence_sb_hrs_rf_sb (preRestrict pre {}) empty_witness = {}"
+unfolding sw_fence_sb_hrs_rf_sb_def
+by simp
+
+lemma sw_fence_sb_hrs_rf_empty [simp]:
+  shows "sw_fence_sb_hrs_rf (preRestrict pre {}) empty_witness = {}"
+unfolding sw_fence_sb_hrs_rf_def
+by simp
+
+lemma sw_fence_rs_rf_sb_empty [simp]:
+  shows "sw_fence_rs_rf_sb (preRestrict pre {}) empty_witness = {}"
+unfolding sw_fence_rs_rf_sb_def
+by simp
+
+lemma release_acquire_fenced_synchronizes_with_set_empty [simp]:
+  shows "release_acquire_fenced_synchronizes_with_set_alt (preRestrict pre {}) empty_witness = {}"
+unfolding release_acquire_fenced_synchronizes_with_set_alt_def
+by simp
+
+lemma with_consume_dob_set_empty [simp]:
+  shows "with_consume_dob_set_alt (preRestrict pre {}) empty_witness = {}"
+unfolding with_consume_dob_set_alt_def with_consume_dob_set_def
+by simp
+
+lemma ithb_r_empty [simp]:
+  shows "inter_thread_happens_before_r (preRestrict pre {}) empty_witness = {}"
+unfolding inter_thread_happens_before_r_def
+by simp
+
+lemma ithb_step_empty [simp]:
+  shows "inter_thread_happens_before_step (preRestrict pre {}) empty_witness = {}"
+unfolding inter_thread_happens_before_step_def
+by simp
+
+lemma ithb_empty [simp]:
+  shows "inter_thread_happens_before_alt (preRestrict pre {}) empty_witness = {}"
+unfolding inter_thread_happens_before_alt_def
+by simp
+
+lemma happens_before_empty [simp]:
+  shows "happens_before s {} {} = {}"
+unfolding happens_before_def
+by simp
+
+lemma getHb_empty [simp]:
+  shows "getHb (preRestrict pre {}) empty_witness = {}"
+unfolding getHb_def
+by simp
+
+lemma getVse_empty [simp]:
+  shows "getVse (preRestrict pre {}) empty_witness = {}"
+unfolding getVse_def
+by simp
+
+subsubsection {* Sb in hb *}
+
+(* Sb in hb in the rel-acq-rlx fragment *)
+
+lemma sbInHb_release_acquire_relaxed_hb:
+  shows "sb pre \<subseteq> release_acquire_relaxed_hb pre wit"
+unfolding release_acquire_relaxed_hb_def no_consume_hb_def
+by auto
+
+(* Sb in hb in the rel-acq-rlx-fence fragment *)
+
+lemma sbInHb_release_acquire_fenced_hb:
+  shows "sb pre \<subseteq> release_acquire_fenced_hb pre wit"
+unfolding release_acquire_fenced_hb_def no_consume_hb_def
+by auto
+
+(* Sb in hb in the with_consume fragment *)
+
+lemma sbInHb_with_consume_hb:
+  shows "sb pre \<subseteq> with_consume_hb pre wit"
+unfolding with_consume_hb_def happens_before_def
+by simp
+
+subsubsection {* Syncing locks *}
+
+(* Syncing locks in hb in the rel-acq-rlx fragment *)
+
+(* To enable reuse between fragments, we isolated the properties that depend on hb. *)
+
+type_synonym hbCalculation = "pre_execution \<Rightarrow> execution_witness \<Rightarrow> (action * action) set"
+
+definition otherThreadLoInHb :: "hbCalculation \<Rightarrow> bool" where 
+  "otherThreadLoInHb hbCalc \<equiv> \<forall>a b pre wit. tid_of a \<noteq> tid_of b \<longrightarrow> 
+                                             is_unlock a \<longrightarrow> 
+                                             is_lock b \<longrightarrow> 
+                                             a \<in> actions0 pre \<longrightarrow> 
+                                             b \<in> actions0 pre \<longrightarrow> 
+                                             (a, b) \<in> lo wit \<longrightarrow> 
+                                             (a, b) \<in> hbCalc pre wit"
+
+definition hbCalcRespectsSyncingLocks  :: "hbCalculation \<Rightarrow> bool" where 
+   "hbCalcRespectsSyncingLocks hbCalc = (\<forall> pre0. \<forall> wit. 
+          well_formed_threads_opsem (pre0, wit, [])
+      \<longrightarrow> locks_only_consistent_lo (pre0, wit, [((''hb''), hbCalc pre0 wit)])
+      \<longrightarrow> (\<forall> a. \<forall> b.     (is_unlock a \<and> is_lock b \<and> (a, b) \<in> lo wit)
+                     \<longrightarrow> (a, b) \<in> hbCalc pre0 wit))"
+
+lemma otherThreadLoInHb_release_acquire_relaxed_hb:
+  shows   "otherThreadLoInHb release_acquire_relaxed_hb"
+unfolding otherThreadLoInHb_def
+          release_acquire_relaxed_hb_def 
+          no_consume_hb_def
+          release_acquire_relaxed_synchronizes_with_set_alt_def
+          sw_lock_def
+by auto
+
+lemma loInHb_aux:
+  assumes well_formed_threads:      "well_formed_threads_opsem (pre, wit, [])"
+      and locks_only_consistent_lo: "locks_only_consistent_lo (pre, wit, [(''hb'', hbCalc pre wit)])"
+      and otherThreadLoInHb:        "otherThreadLoInHb hbCalc"
+      and sbInHb:                   "sb pre \<subseteq> hbCalc pre wit"
+      and is_lo:                    "is_unlock a" "is_lock b" "(a, b) \<in> lo wit"
+  shows                             "(a, b) \<in> hbCalc pre wit"
+proof -
+
+  have "relOver (lo wit) (actions0 pre)"
+    using locks_only_consistent_lo by auto
+  hence in_actions: "a \<in> actions0 pre" "b \<in> actions0 pre" 
+    using is_lo unfolding relOver_def by auto
+
+  show "(a, b) \<in> hbCalc pre wit" 
+    proof (cases "tid_of a = tid_of b")
+      assume "tid_of a \<noteq> tid_of b"
+      thus "(a, b) \<in> hbCalc pre wit"
+        using otherThreadLoInHb in_actions is_lo
+        unfolding otherThreadLoInHb_def
+        by simp
+    next
+      assume tid_eq: "tid_of a = tid_of b"
+
+      have "(b, a) \<notin> hbCalc pre wit" 
+        using locks_only_consistent_lo is_lo by auto
+      hence "(b, a) \<notin> sb pre" 
+        using sbInHb by auto
+
+      have "a \<noteq> b" 
+        using locks_only_consistent_lo is_lo by auto
+
+      have "is_at_mutex_location (lk pre) a" 
+        using assms is_lo in_actions by auto
+      hence not_na_loc: "\<not> is_at_non_atomic_location (lk pre) a"
+        by auto
+
+      have "indeterminate_sequencing pre" 
+        using well_formed_threads by auto
+      hence "(a, b) \<in> sb pre"
+        unfolding indeterminate_sequencing_def
+        using in_actions tid_eq `a \<noteq> b` not_na_loc `(b, a) \<notin> sb pre`
+        by auto
+
+      thus "(a, b) \<in> hbCalc pre wit"
+        using sbInHb by auto
+
+    qed
+qed
+
+lemma loInHb_release_acquire_relaxed_hb:
+  shows "hbCalcRespectsSyncingLocks release_acquire_relaxed_hb"
+unfolding hbCalcRespectsSyncingLocks_def
+using sbInHb_release_acquire_relaxed_hb 
+      otherThreadLoInHb_release_acquire_relaxed_hb
+      loInHb_aux
+by metis
+
+(* Syncing locks in hb in the rel-acq-rlx-fence fragment *)
+
+lemma otherThreadLoInHb_release_acquire_fenced_hb:
+  shows   "otherThreadLoInHb release_acquire_fenced_hb"
+unfolding otherThreadLoInHb_def
+          release_acquire_fenced_hb_def 
+          no_consume_hb_def
+          release_acquire_fenced_synchronizes_with_set_alt_def
+          sw_lock_def
+by auto
+
+lemma loInHb_release_acquire_fenced_hb:
+  shows "hbCalcRespectsSyncingLocks release_acquire_fenced_hb"
+unfolding hbCalcRespectsSyncingLocks_def
+using sbInHb_release_acquire_fenced_hb 
+      otherThreadLoInHb_release_acquire_fenced_hb
+      loInHb_aux
+by metis
+
+(* Syncing locks in hb in the with_consume fragment *)
+
+lemma otherThreadLoInHb_with_consume_hb:
+  shows   "otherThreadLoInHb with_consume_hb"
+unfolding otherThreadLoInHb_def
+          with_consume_hb_def 
+          happens_before_def
+          inter_thread_happens_before_alt_def
+          inter_thread_happens_before_step_def
+          inter_thread_happens_before_r_def
+          release_acquire_fenced_synchronizes_with_set_alt_def
+          sw_lock_def
+by auto
+
+lemma loInHb_with_consume_hb:
+  shows "hbCalcRespectsSyncingLocks with_consume_hb"
+unfolding hbCalcRespectsSyncingLocks_def
+using sbInHb_with_consume_hb 
+      otherThreadLoInHb_with_consume_hb
+      loInHb_aux
+by metis
+
+subsubsection {* Monotonicity *}
+
+(* Monotonicity hb in the locks only fragment *)
+
+lemma monotonicity_locks_only_sw:
+  shows   "  locks_only_sw_set_alt (preRestrict pre actions) (incWitRestrict wit actions)
+           \<subseteq> locks_only_sw_set_alt pre wit "
+unfolding locks_only_sw_set_alt_def
+          locks_only_sw_set_def 
+by (auto simp add: locks_only_sw_def)
+
+lemma monotonicity_no_consume_hb:
+  assumes "sw2 \<subseteq> sw"
+      and "p_sb2 \<subseteq> p_sb"
+  shows   "no_consume_hb p_sb2 sw2 \<subseteq> no_consume_hb p_sb sw"
+using assms
+unfolding no_consume_hb_def
+by (metis Un_mono trancl_mono2)
+(* by (metis Un_mono order_refl trancl_mono2) *)
+
+lemma monotonicity_locks_only_hb:
+  shows "  locks_only_hb (preRestrict pre actions) (incWitRestrict wit actions)
+         \<subseteq> locks_only_hb pre wit"
+unfolding locks_only_hb_def 
+using monotonicity_no_consume_hb[OF monotonicity_locks_only_sw]
+by auto
+
+(* Monotonicity hb in the rel-acq fragment *)
+
+lemma monotonicity_release_acquire_sw:
+  shows   "  release_acquire_synchronizes_with_set_alt (preRestrict pre actions) (incWitRestrict wit actions) 
+           \<subseteq> release_acquire_synchronizes_with_set_alt pre wit"
+apply (intro subrelI, elim release_acquire_swIE)
+unfolding sw_asw_def sw_lock_def sw_rel_acq_def
+by auto
+(* by (auto elim: relRestrictE) *)
+
+lemma monotonicity_release_acquire_hb:
+  shows "  release_acquire_hb (preRestrict pre actions) (incWitRestrict wit actions) 
+         \<subseteq> release_acquire_hb pre wit"
+unfolding release_acquire_hb_def 
+using monotonicity_no_consume_hb[OF monotonicity_release_acquire_sw]
+by auto
+
+(* Monotonicity hb in the rel-acq-rlx fragment *)
+
+lemma monotonicity_release_sequence:
+  assumes "downclosed actions (mo wit)"
+          "(a, b) \<in> release_sequence_set_alt (preRestrict pre actions) (incWitRestrict wit actions)"
+          "b \<in> actions"          
+  shows   "(a, b) \<in> release_sequence_set_alt pre wit"
+using assms
+unfolding release_sequence_set_alt_def 
+          release_sequence_set_def
+          downclosed_def
+by auto
+
+lemma monotonicity_sw_rel_acq_rs:
+  assumes "downclosed actions (mo wit)"
+  shows   "  sw_rel_acq_rs (preRestrict pre actions) (incWitRestrict wit actions)
+           \<subseteq> sw_rel_acq_rs pre wit"
+(* TODO: for some reason "cases rule: sw_rel_acq_rsIE" doesn't work after the "intro subrelI". When
+everything is made explicit (the fix, assume, thus) then it does do the right thing. *)
+proof (intro subrelI)
+  fix a b
+  assume "(a, b) \<in> sw_rel_acq_rs (preRestrict pre actions) (incWitRestrict wit actions)"
+  thus   "(a, b) \<in> sw_rel_acq_rs pre wit"
+    proof (cases rule: sw_rel_acq_rsIE)
+      case (rel_acq_rs c)
+      hence "c \<in> actions" by auto (* by (auto elim: relRestrictE) *)
+      hence "(a, c) \<in> release_sequence_set_alt pre wit" 
+        using monotonicity_release_sequence assms rel_acq_rs
+        by metis
+      thus "   a \<in> actions0 pre \<and> b \<in> actions0 pre \<and> c \<in> actions0 pre
+            \<and> (a, c) \<in> release_sequence_set_alt pre wit \<and> (c, b) \<in> rf wit "
+        using rel_acq_rs by auto (* by (auto elim: relRestrictE) *)
+    qed
+qed
+
+lemma monotonicity_release_acquire_relaxed_sw:
+  assumes downclosed: "downclosed actions (mo wit)"
+  shows   "  release_acquire_relaxed_synchronizes_with_set_alt (preRestrict pre actions) (incWitRestrict wit actions)
+           \<subseteq> release_acquire_relaxed_synchronizes_with_set_alt pre wit"
+using monotonicity_sw_rel_acq_rs[OF downclosed]
+by (intro subrelI, elim release_acquire_relaxed_swIE)
+   (auto intro!: sw_aswI sw_lockI)
+(* by (intro subrelI, elim release_acquire_relaxed_swIE)
+   (auto elim!: sw_lockE sw_aswE 
+         intro!: sw_aswI sw_lockI 
+         elim: relRestrictE) *)
+
+lemma monotonicity_release_acquire_relaxed_hb:
+  assumes downclosed_mo: "downclosed actions (mo wit)"
+  shows   "  release_acquire_relaxed_hb (preRestrict pre actions) (incWitRestrict wit actions)
+           \<subseteq> release_acquire_relaxed_hb pre wit"
+unfolding release_acquire_relaxed_hb_def 
+using monotonicity_no_consume_hb[OF monotonicity_release_acquire_relaxed_sw[OF downclosed_mo]]
+by auto
+
+(* Monotonicity hb in the rel-acq-rlx-fenced fragment *)
+
+lemma monotonicity_hypothetical_release_sequence:
+  assumes "downclosed actions (mo wit)"
+          "(a, b) \<in> hypothetical_release_sequence_set_alt (preRestrict pre actions) (incWitRestrict wit actions)"
+          "b \<in> actions"          
+  shows   "(a, b) \<in> hypothetical_release_sequence_set_alt pre wit"
+using assms
+unfolding hypothetical_release_sequence_set_alt_def 
+          hypothetical_release_sequence_set_def
+          downclosed_def
+by auto
+
+lemma monotonicity_sw_fence_sb_hrs_rf_sb:
+  assumes downclosed: "downclosed actions (mo wit)"
+  shows   "  sw_fence_sb_hrs_rf_sb (preRestrict pre actions) (incWitRestrict wit actions)
+           \<subseteq> sw_fence_sb_hrs_rf_sb pre wit"
+proof (intro subrelI)
+  fix a b
+  assume "(a, b) \<in> sw_fence_sb_hrs_rf_sb (preRestrict pre actions) (incWitRestrict wit actions)"
+  thus "(a, b) \<in> sw_fence_sb_hrs_rf_sb pre wit"
+    proof (cases rule: sw_fence_sb_hrs_rf_sbIE)
+      let ?hrs  = "hypothetical_release_sequence_set_alt pre wit"
+      case (fence x y z)
+      hence "y \<in> actions" by auto (* by (auto elim: relRestrictE) *)
+      hence "(x, y) \<in> ?hrs"
+        using monotonicity_hypothetical_release_sequence
+        using downclosed fence
+        by auto
+      thus "  a \<in> actions0 pre \<and> b \<in> actions0 pre \<and> x \<in> actions0 pre
+            \<and> y \<in> actions0 pre \<and> z \<in> actions0 pre
+            \<and> (a, x) \<in> sb pre \<and> (x, y) \<in> ?hrs \<and> (y, z) \<in> rf wit \<and> (z, b) \<in> sb pre"
+        using fence by auto (* by (auto elim: relRestrictE) *)
+    qed
+qed
+
+lemma monotonicity_sw_fence_sb_hrs_rf:
+  assumes downclosed: "downclosed actions (mo wit)"
+  shows   "  sw_fence_sb_hrs_rf (preRestrict pre actions) (incWitRestrict wit actions)
+           \<subseteq> sw_fence_sb_hrs_rf pre wit"
+proof (intro subrelI)
+  fix a b
+  assume "(a, b) \<in> sw_fence_sb_hrs_rf (preRestrict pre actions) (incWitRestrict wit actions)"
+  thus "(a, b) \<in> sw_fence_sb_hrs_rf pre wit"
+    proof (cases rule: sw_fence_sb_hrs_rfIE)
+      let ?hrs  = "hypothetical_release_sequence_set_alt pre wit"
+      case (fence x y)
+      hence "y \<in> actions" by auto (* by (auto elim: relRestrictE) *)
+      hence "(x, y) \<in> ?hrs"
+        using monotonicity_hypothetical_release_sequence
+        using downclosed fence
+        by auto
+      thus "  a \<in> actions0 pre \<and> b \<in> actions0 pre \<and> x \<in> actions0 pre
+            \<and> y \<in> actions0 pre \<and> (a, x) \<in> sb pre \<and> (x, y) \<in> ?hrs \<and> (y, b) \<in> rf wit"
+        using fence by auto (* by (auto elim: relRestrictE) *)
+    qed
+qed
+
+lemma monotonicity_sw_fence_rs_rf_sb:
+  assumes downclosed: "downclosed actions (mo wit)"
+  shows   "  sw_fence_rs_rf_sb (preRestrict pre actions) (incWitRestrict wit actions)
+           \<subseteq> sw_fence_rs_rf_sb pre wit"
+proof (intro subrelI)
+  fix a b
+  assume "(a, b) \<in> sw_fence_rs_rf_sb (preRestrict pre actions) (incWitRestrict wit actions)"
+  thus "(a, b) \<in> sw_fence_rs_rf_sb pre wit"
+    proof (cases rule: sw_fence_rs_rf_sbIE)
+      let ?rs  = "release_sequence_set_alt pre wit"
+      case (fence x y)
+      hence "y \<in> actions" by auto (* by (auto elim: relRestrictE) *)
+      hence "(a, x) \<in> ?rs"
+        using monotonicity_release_sequence
+        using downclosed fence
+        by auto (* by (auto elim: relRestrictE) *)
+      thus "  a \<in> actions0 pre \<and> b \<in> actions0 pre \<and> x \<in> actions0 pre 
+            \<and> y \<in> actions0 pre \<and> (a, x) \<in> ?rs \<and> (x, y) \<in> (rf wit) \<and> (y, b) \<in> (sb pre)"
+        using fence by auto (* by (auto elim: relRestrictE) *)
+    qed
+qed
+
+lemma monotonicity_release_acquire_fenced_sw: 
+  assumes downclosed: "downclosed actions (mo wit)"
+  shows   "  release_acquire_fenced_synchronizes_with_set_alt (preRestrict pre actions) (incWitRestrict wit actions)
+           \<subseteq> release_acquire_fenced_synchronizes_with_set_alt pre wit"
+using monotonicity_sw_fence_sb_hrs_rf_sb[OF downclosed]
+using monotonicity_sw_fence_sb_hrs_rf[OF downclosed]
+using monotonicity_sw_fence_rs_rf_sb[OF downclosed]
+using monotonicity_sw_rel_acq_rs[OF downclosed]
+apply (intro subrelI, elim release_acquire_fenced_swIE)
+by (auto 8 2 intro!: sw_aswI sw_lockI)
+(* 
+by (auto 8 2 elim!: sw_lockE sw_aswE 
+             intro!: sw_aswI sw_lockI) *)
+
+lemma monotonicity_release_acquire_fenced_hb:
+  assumes "downclosed actions (mo wit)"
+  shows   "  release_acquire_fenced_hb (preRestrict pre actions) (incWitRestrict wit actions)
+           \<subseteq> release_acquire_fenced_hb pre wit"
+unfolding release_acquire_fenced_hb_def 
+using monotonicity_no_consume_hb[OF monotonicity_release_acquire_fenced_sw[OF assms]]
+by auto
+
+(* Monotonicity hb in the with_consume fragment *)
+
+lemma monotonicity_with_consume_cad:
+  shows "with_consume_cad_set_alt (preRestrict pre actions) (incWitRestrict wit actions) \<subseteq> 
+         with_consume_cad_set_alt pre wit"
+unfolding with_consume_cad_set_alt_def
+          with_consume_cad_set_def
+by (intro trancl_mono2) auto
+
+lemma monotonicity_with_consume_dob_set:
+  assumes downclosed: "downclosed actions (mo wit)"
+  shows "  with_consume_dob_set_alt (preRestrict pre actions) (incWitRestrict wit actions)
+         \<subseteq> with_consume_dob_set_alt pre wit"
+proof (intro subrelI)
+  let ?rs   = "release_sequence_set_alt pre wit"
+  let ?rs2  = "release_sequence_set_alt (preRestrict pre actions) (incWitRestrict wit actions)"
+  let ?cad  = "with_consume_cad_set_alt pre wit"
+  let ?cad2 = "with_consume_cad_set_alt (preRestrict pre actions) (incWitRestrict wit actions)"
+  fix a b
+  assume in_dob: "(a, b) \<in> with_consume_dob_set_alt (preRestrict pre actions) (incWitRestrict wit actions)"
+  obtain ba e where ba_e: "ba \<in> actions0 pre \<and> 
+                           is_consume ba \<and> 
+                           e \<in> actions0 pre \<and> 
+                           (a, e) \<in> ?rs2 \<and> 
+                           (e, ba) \<in> relRestrict (rf wit) actions \<and> 
+                           ((ba, b) \<in> ?cad2 \<or> ba = b)"
+    using in_dob
+    unfolding with_consume_dob_set_alt_def
+              with_consume_dob_set_def
+    by (auto simp add: dependency_ordered_before_def)
+  hence "e \<in> actions" unfolding relRestrict_def by auto
+  hence rs: "(a, e) \<in> ?rs"
+    using ba_e monotonicity_release_sequence[OF downclosed]
+    by fast
+  have cad2: "(ba, b) \<in> ?cad \<or> ba = b" 
+    using ba_e monotonicity_with_consume_cad by auto
+  show "(a, b) \<in> with_consume_dob_set_alt pre wit"
+    using in_dob
+    unfolding with_consume_dob_set_alt_def
+              with_consume_dob_set_def
+    using ba_e rs cad2 
+    by (auto simp add: dependency_ordered_before_def)
+qed
+
+lemma relComp_member:
+  shows "(a, c) \<in> relcomp r r' = (\<exists>b. (a, b) \<in> r \<and> (b, c) \<in> r')"
+by auto
+
+lemma monotonicity_ithb:
+  assumes downclosed: "downclosed actions (mo wit)"
+  shows   "  inter_thread_happens_before_alt (preRestrict pre actions) (incWitRestrict wit actions)
+           \<subseteq> inter_thread_happens_before_alt pre wit"
+unfolding inter_thread_happens_before_alt_def
+          inter_thread_happens_before_step_def
+          inter_thread_happens_before_r_def
+          Let_def
+using monotonicity_release_acquire_fenced_sw[OF downclosed]
+using monotonicity_with_consume_dob_set[OF downclosed]
+by (auto intro!: trancl_mono2 Un_mono relcomp_mono del: subsetI)
+
+lemma monotonicity_with_consume_hb:
+  assumes downclosed: "downclosed actions (mo wit)"
+  shows   "  with_consume_hb (preRestrict pre actions) (incWitRestrict wit actions)
+           \<subseteq> with_consume_hb pre wit"
+unfolding with_consume_hb_def happens_before_def
+using monotonicity_ithb[OF downclosed]
+by auto
+
+subsubsection {* Prefixes are final *}
+
+(* Prefixes are final in the rel-acq-rlx fragment *)
+
+(* TODO: the following defintions can be refactored into something simpler. *)
+
+definition prefixes_are_final  :: "(action)set \<Rightarrow>(action*action)set \<Rightarrow>(action*action)set \<Rightarrow> bool "  where 
+  "prefixes_are_final s r r' = (\<forall> (a, b) \<in> r. b \<in> s \<longrightarrow> (a, b) \<in> r')"
+
+definition selective_prefixes_are_final  :: "(action \<Rightarrow> bool)\<Rightarrow>(action)set \<Rightarrow>(action*action)set \<Rightarrow>(action*action)set \<Rightarrow> bool "  where 
+  "selective_prefixes_are_final f s r r' = (\<forall> (a, b) \<in> r. (b \<in> s \<and> f b) \<longrightarrow> (a, b) \<in> r')"
+
+definition sbMinus  :: " pre_execution \<Rightarrow>(action*action)set \<Rightarrow>(action*action)set "  where 
+  "sbMinus pre1 rel = (set_filter (\<lambda> (a, b). (is_na_or_non_write pre1 b)) rel)"
+ 
+definition selective_downclosed  :: "(action \<Rightarrow> bool)\<Rightarrow>(action)set \<Rightarrow>(action*action)set \<Rightarrow> bool "  where 
+  "selective_downclosed f s r = (\<forall> (a, b) \<in> r. (b \<in> s \<and> f b) \<longrightarrow> (a \<in> s))"
+
+definition hbCalcIsFinalForPrefixes  :: "(pre_execution \<Rightarrow> execution_witness \<Rightarrow>(action*action)set)\<Rightarrow> bool "  where 
+  "hbCalcIsFinalForPrefixes hbCalc = (\<forall> pre0. \<forall> wit. \<forall> actions1.  
+            downclosed actions1 (rf wit)
+          \<and> downclosed actions1 (mo wit)
+          \<and> downclosed actions1 (sbMinus pre0 (sb pre0))
+          \<and> trans (sb pre0)
+          \<and> dd pre0 \<subseteq> sb pre0
+          \<and> selective_downclosed (is_na_or_non_write pre0) actions1 (hbCalc pre0 wit)
+     \<longrightarrow>  selective_prefixes_are_final (is_na_or_non_write pre0)
+                                   actions1
+                                   (hbCalc pre0 wit) 
+                                   (hbCalc (preRestrict pre0 actions1) (incWitRestrict wit actions1)))"
+
+definition hbCalcIsMonotonic  :: "(pre_execution \<Rightarrow> execution_witness \<Rightarrow>(action*action)set)\<Rightarrow> bool "  where 
+  "hbCalcIsMonotonic hbCalc = (\<forall> pre0. \<forall> wit. \<forall> actions1.
+          downclosed actions1 (mo wit) 
+     \<longrightarrow>  hbCalc (preRestrict pre0 actions1) (incWitRestrict wit actions1) \<subseteq> hbCalc pre0 wit)"
+
+lemma final_release_sequence:
+  assumes  "downclosed actions (mo wit)"
+      and  "b \<in> actions"
+      and  "(a, b) \<in> release_sequence_set_alt pre wit"
+  shows    "  a \<in> actions
+            \<and> (a, b) \<in> release_sequence_set_alt (preRestrict pre actions) (incWitRestrict wit actions)"
+using assms
+unfolding release_sequence_set_alt_def 
+          release_sequence_set_def 
+          downclosed_def
+by auto
+
+lemma final_sw_asw:
+  assumes "(a, b) \<in> sw_asw pre wit"
+      and "a \<in> actions" 
+      and "b \<in> actions"
+  shows   "(a, b) \<in> sw_asw (preRestrict pre actions) (incWitRestrict wit actions)"
+using assms
+unfolding sw_asw_def
+by auto
+
+lemma final_sw_lock:
+  assumes "(a, b) \<in> sw_lock pre wit"
+      and "a \<in> actions" 
+      and "b \<in> actions"
+  shows   "(a, b) \<in> sw_lock (preRestrict pre actions) (incWitRestrict wit actions)"
+using assms
+unfolding sw_lock_def
+by auto
+
+lemma final_sw_rel_acq_rs:
+  assumes "(a, b) \<in> sw_rel_acq_rs pre wit"
+      and downclosed_rf: "downclosed actions (rf wit)"
+      and downclosed_mo: "downclosed actions (mo wit)"
+      and "b \<in> actions"
+  shows   "(a, b) \<in> sw_rel_acq_rs (preRestrict pre actions) (incWitRestrict wit actions)"
+using assms(1)
+proof (cases rule: sw_rel_acq_rsIE, simp)
+  case (rel_acq_rs c)
+  hence "c \<in> actions" 
+    using downclosed_rf `b \<in> actions` by (auto elim: downclosedE)
+  let ?rs   = "release_sequence_set_alt pre wit"
+  let ?rs2  = "release_sequence_set_alt (preRestrict pre actions) (incWitRestrict wit actions)"
+  have "a \<in> actions \<and> (a, c) \<in> ?rs2"
+    using final_release_sequence[OF downclosed_mo `c \<in> actions`]
+    using rel_acq_rs
+    by auto
+  (* TODO: I have no idea why the simplifier did not get rid of the double occurrences. *)
+  thus "a \<in> actions \<and> b \<in> actions \<and> c \<in> actions \<and> (a, c) \<in> ?rs2 \<and> c \<in> actions \<and> b \<in> actions"
+    using rel_acq_rs `b \<in> actions` `c \<in> actions` by auto
+qed
+
+lemma final_release_acquire_relaxed_sw:
+  assumes downclosed_rf: "downclosed actions (rf wit)"
+      and downclosed_mo: "downclosed actions (mo wit)"
+      and "a \<in> actions" 
+      and "b \<in> actions"
+      and sw1: "(a, b) \<in> release_acquire_relaxed_synchronizes_with_set_alt pre wit"
+  shows   "(a, b) \<in> release_acquire_relaxed_synchronizes_with_set_alt (preRestrict pre actions) (incWitRestrict wit actions)"
+using sw1
+apply (cases rule: release_acquire_relaxed_swIE)
+using final_sw_asw[OF _ `a \<in> actions` `b \<in> actions`]
+      final_sw_lock[OF _ `a \<in> actions` `b \<in> actions`]
+      final_sw_rel_acq_rs[OF _ downclosed_rf downclosed_mo `b \<in> actions`]
+by metis+
+
+lemma final_no_consume_hb_aux:
+  assumes downclosed_rf: "downclosed actions (rf wit)"
+      and downclosed_mo: "downclosed actions (mo wit)"
+      and                "b \<in> actions"
+      and downclosed_hb: "\<And>c. (c, b) \<in> (no_consume_hb p_sb sw) \<Longrightarrow> c \<in> actions"
+      and in_hb:         "(a, b) \<in> no_consume_hb p_sb sw"
+      and final_sw:      "\<And>x y. \<lbrakk>x \<in> actions; y \<in> actions; (x, y) \<in> sw\<rbrakk> \<Longrightarrow> (x, y) \<in> sw'"
+  shows   "(a, b) \<in> no_consume_hb (relRestrict p_sb actions) sw'"
+proof -
+  let ?hb = "no_consume_hb p_sb sw"
+  let ?p_sb' = "relRestrict p_sb actions"
+  have "(a, b) \<in> (p_sb \<union> sw)\<^sup>+" using in_hb unfolding no_consume_hb_def .
+  hence "(a, b) \<in> (?p_sb' \<union> sw')\<^sup>+"    
+    proof (rule converse_trancl_induct)
+      fix y
+      assume inSbSw: "(y, b) \<in> p_sb \<union> sw"
+      hence "(y, b) \<in> ?hb" unfolding no_consume_hb_def by auto
+      hence "y \<in> actions" using downclosed_hb by simp
+      hence "(y, b) \<in> ?p_sb' \<union> sw'"
+        using final_sw `b \<in> actions` inSbSw 
+        by auto
+      thus "(y, b) \<in> (?p_sb' \<union> sw')\<^sup>+" by auto
+    next
+      fix y z
+      assume inSbSw:        "(y, z) \<in> p_sb \<union> sw"
+         and inSbSwTrancl:  "(z, b) \<in> (p_sb \<union> sw)\<^sup>+"
+         and inSbSw2Trancl: "(z, b) \<in> (?p_sb' \<union> sw')\<^sup>+"
+      hence "(z, b) \<in> ?hb" unfolding no_consume_hb_def by auto
+      hence "z \<in> actions" using downclosed_hb by simp
+      have "(y, b) \<in> ?hb"
+        unfolding no_consume_hb_def
+        using inSbSw inSbSwTrancl
+        by (rule trancl_into_trancl2)
+      hence "y \<in> actions" using downclosed_hb by simp
+      hence "(y, z) \<in> ?p_sb' \<union> sw'"
+        using final_sw inSbSw `z \<in> actions`
+        by auto     
+      thus "(y, b) \<in> (?p_sb' \<union> sw')\<^sup>+" 
+        using inSbSw2Trancl
+        by (rule trancl_into_trancl2)
+    qed
+  thus "(a, b) \<in> no_consume_hb ?p_sb' sw'" 
+    unfolding no_consume_hb_def
+    by simp
+qed
+
+lemma final_no_consume_hb:
+  fixes pre wit sw sw' actions
+  defines "hb  \<equiv> no_consume_hb (sb pre) sw"
+      and "hb' \<equiv> no_consume_hb (relRestrict (sb pre) actions) sw'"
+  assumes downclosed_rf: "downclosed actions (rf wit)"
+      and downclosed_mo: "downclosed actions (mo wit)"
+      and downclosed_hb:  "selective_downclosed f actions hb"
+      and final_sw:      "\<And>x y. \<lbrakk>x \<in> actions; y \<in> actions; (x, y) \<in> sw\<rbrakk> \<Longrightarrow> (x, y) \<in> sw'"
+  shows   "selective_prefixes_are_final f actions hb hb'"
+unfolding selective_prefixes_are_final_def
+proof auto
+  fix a b
+  assume "b \<in> actions" "f b" "(a, b) \<in> hb"
+  hence "\<And>d. (d, b) \<in> hb \<Longrightarrow> d \<in> actions"
+    using downclosed_hb unfolding selective_downclosed_def by auto
+  thus "(a, b) \<in> hb'" 
+    using `(a, b) \<in> hb` final_sw
+    unfolding hb_def hb'_def
+    using final_no_consume_hb_aux[OF downclosed_rf downclosed_mo  `b \<in> actions`]
+    by metis
+qed
+
+lemma final_release_acquire_relaxed_hb:
+  shows "hbCalcIsFinalForPrefixes release_acquire_relaxed_hb"
+unfolding hbCalcIsFinalForPrefixes_def
+proof auto
+  fix pre :: pre_execution
+  fix wit :: execution_witness
+  fix actions
+  let ?sw  = "release_acquire_relaxed_synchronizes_with_set_alt pre wit"
+  let ?sw2 = "release_acquire_relaxed_synchronizes_with_set_alt (preRestrict pre actions) (incWitRestrict wit actions)"
+  let ?f   = "is_na_or_non_write pre"
+  assume downclosed_rf: "downclosed actions (rf wit)" 
+     and downclosed_mo: "downclosed actions (mo wit)"
+     and downclosed_sb: "downclosed actions (sbMinus pre (sb pre))"
+     and downclosed_hb: "selective_downclosed ?f actions (release_acquire_relaxed_hb pre wit)"
+  have final_sw: "\<And>x y. \<lbrakk>x \<in> actions; y \<in> actions; (x, y) \<in> ?sw\<rbrakk> \<Longrightarrow> (x, y) \<in> ?sw2"
+    using final_release_acquire_relaxed_sw[OF downclosed_rf downclosed_mo]
+    by metis 
+  show "selective_prefixes_are_final (is_na_or_non_write pre) 
+                                     actions
+                                     (release_acquire_relaxed_hb pre wit) 
+                                     (release_acquire_relaxed_hb (preRestrict pre actions) (incWitRestrict wit actions))"
+    using final_no_consume_hb[OF downclosed_rf downclosed_mo _ final_sw] downclosed_hb
+    unfolding release_acquire_relaxed_hb_def
+    by auto
+qed
+
+(* Prefixes are final in the rel-acq-rlx-fence fragment *)
+
+lemma final_hypothetical_release_sequence:
+  assumes  "downclosed actions (mo wit)"
+      and  "b \<in> actions"
+      and  "(a, b) \<in> hypothetical_release_sequence_set_alt pre wit"
+  shows   "  a \<in> actions 
+           \<and> (a, b) \<in> hypothetical_release_sequence_set_alt (preRestrict pre actions) (incWitRestrict wit actions)"
+using assms
+unfolding hypothetical_release_sequence_set_alt_def 
+          hypothetical_release_sequence_set_def 
+          downclosed_def
+by auto
+
+lemma final_sw_fence_sb_hrs_rf_sb:
+  assumes "(a, b) \<in> sw_fence_sb_hrs_rf_sb pre wit"
+      and downclosed_rf: "downclosed actions (rf wit)"
+      and downclosed_mo: "downclosed actions (mo wit)"
+      and downclosed_sb: "downclosed actions (sbMinus pre (sb pre))"
+      and "a \<in> actions"
+      and "b \<in> actions"
+  shows   "(a, b) \<in> sw_fence_sb_hrs_rf_sb (preRestrict pre actions) (incWitRestrict wit actions)"
+using assms(1)
+proof (cases rule: sw_fence_sb_hrs_rf_sbIE, simp)
+  let ?hrs  = "hypothetical_release_sequence_set_alt pre wit"
+  let ?hrs2  = "hypothetical_release_sequence_set_alt (preRestrict pre actions) (incWitRestrict wit actions)"
+  case (fence x y z)
+  have "is_na_or_non_write pre b" 
+    using `is_fence b` unfolding is_na_or_non_write_def by (cases b) auto
+  hence "(z, b) \<in> sbMinus pre (sb pre)" 
+    using `(z, b) \<in> sb pre` unfolding sbMinus_def by auto
+  hence "z \<in> actions" 
+    using downclosed_sb `b \<in> actions` unfolding downclosed_def by metis  
+  hence "y \<in> actions"
+    using downclosed_rf `(y, z) \<in> rf wit` unfolding downclosed_def by metis  
+  hence "x \<in> actions \<and> (x, y) \<in> ?hrs2"
+    using final_hypothetical_release_sequence `(x, y) \<in> ?hrs` downclosed_mo
+    by metis
+  (* TODO: No idea why the simplifier left the double conjuncts. *)
+  thus "  a \<in> actions \<and> b \<in> actions \<and> x \<in> actions \<and> y \<in> actions \<and> z \<in> actions \<and> a \<in> actions
+        \<and> x \<in> actions \<and> (x, y) \<in> ?hrs2 \<and> y \<in> actions \<and> z \<in> actions \<and> b \<in> actions"
+    using fence `z \<in> actions` `y \<in> actions` `a \<in> actions` `b \<in> actions` by auto
+qed
+
+lemma final_sw_fence_sb_hrs_rf:
+  assumes "(a, b) \<in> sw_fence_sb_hrs_rf pre wit"
+      and downclosed_rf: "downclosed actions (rf wit)"
+      and downclosed_mo: "downclosed actions (mo wit)"
+      and "a \<in> actions"
+      and "b \<in> actions"
+  shows   "(a, b) \<in> sw_fence_sb_hrs_rf (preRestrict pre actions) (incWitRestrict wit actions)"
+using assms(1)
+proof (cases rule: sw_fence_sb_hrs_rfIE, simp)
+  let ?hrs  = "hypothetical_release_sequence_set_alt pre wit"
+  let ?hrs2  = "hypothetical_release_sequence_set_alt (preRestrict pre actions) (incWitRestrict wit actions)"
+  case (fence x y)
+  have "y \<in> actions" 
+    using downclosed_rf `b \<in> actions` `(y, b) \<in> rf wit` 
+    unfolding downclosed_def by metis
+  hence "x \<in> actions \<and> (x, y) \<in> ?hrs2" 
+    using final_hypothetical_release_sequence `(x, y) \<in> ?hrs` downclosed_mo
+    by metis
+  thus "  a \<in> actions \<and> b \<in> actions \<and> x \<in> actions \<and> y \<in> actions \<and> a \<in> actions \<and> x \<in> actions 
+        \<and> (x, y) \<in> ?hrs2 \<and> y \<in> actions \<and> b \<in> actions"
+    using fence `y \<in> actions` `a \<in> actions` `b \<in> actions` by auto
+qed
+
+lemma final_sw_fence_rs_rf_sb:
+  assumes "(a, b) \<in> sw_fence_rs_rf_sb pre wit"
+      and downclosed_rf: "downclosed actions (rf wit)"
+      and downclosed_mo: "downclosed actions (mo wit)"
+      and downclosed_sb: "downclosed actions (sbMinus pre (sb pre))"
+      and b: "b \<in> actions"
+  shows   "(a, b) \<in> sw_fence_rs_rf_sb (preRestrict pre actions) (incWitRestrict wit actions)"
+using assms(1)
+proof (cases rule: sw_fence_rs_rf_sbIE, simp)
+  let ?rs  = "release_sequence_set_alt pre wit"
+  let ?rs2  = "release_sequence_set_alt (preRestrict pre actions) (incWitRestrict wit actions)"
+  case (fence x y)
+  have "is_na_or_non_write pre b" 
+    using `is_fence b` unfolding is_na_or_non_write_def by (cases b) auto
+  hence "(y, b) \<in> sbMinus pre (sb pre)" 
+    using `(y, b) \<in> sb pre` unfolding sbMinus_def by auto
+  hence "y \<in> actions" 
+    using downclosed_sb b unfolding downclosed_def by metis
+  hence "x \<in> actions"
+    using downclosed_rf `(x, y) \<in> rf wit` unfolding downclosed_def by metis
+  hence "a \<in> actions \<and> (a, x) \<in> ?rs2" 
+    using final_release_sequence `(a, x) \<in> ?rs` downclosed_mo
+    by metis
+  thus "  a \<in> actions \<and> b \<in> actions \<and> x \<in> actions \<and> y \<in> actions
+        \<and> (a, x) \<in> ?rs2 \<and> x \<in> actions \<and> y \<in> actions \<and> b \<in> actions"
+    using fence `x \<in> actions` `y \<in> actions` `b \<in> actions` by auto
+qed
+
+lemma final_release_acquire_fenced_sw:
+  assumes downclosed_rf: "downclosed actions (rf wit)"
+      and downclosed_mo: "downclosed actions (mo wit)"
+      and downclosed_sb: "downclosed actions (sbMinus pre (sb pre))"
+      and "a \<in> actions"
+      and "b \<in> actions"
+      and sw1: "(a, b) \<in> release_acquire_fenced_synchronizes_with_set_alt pre wit"
+  shows   "(a, b) \<in> release_acquire_fenced_synchronizes_with_set_alt (preRestrict pre actions) (incWitRestrict wit actions)"
+using sw1
+apply (cases rule: release_acquire_fenced_swIE)
+using final_sw_asw
+      final_sw_lock
+      final_sw_rel_acq_rs
+      final_sw_fence_sb_hrs_rf_sb
+      final_sw_fence_sb_hrs_rf
+      final_sw_fence_rs_rf_sb
+      assms
+by metis+
+
+lemma final_release_acquire_fenced_hb:
+  shows "hbCalcIsFinalForPrefixes release_acquire_fenced_hb"
+unfolding hbCalcIsFinalForPrefixes_def 
+proof auto
+  fix pre :: pre_execution
+  fix wit :: execution_witness
+  fix actions
+  let ?sw   = "release_acquire_fenced_synchronizes_with_set_alt pre wit"
+  let ?sw2  = "release_acquire_fenced_synchronizes_with_set_alt (preRestrict pre actions) (incWitRestrict wit actions)"
+  let ?f    = "is_na_or_non_write pre"
+  assume downclosed_rf: "downclosed actions (rf wit)" 
+     and downclosed_mo: "downclosed actions (mo wit)"
+     and downclosed_sb: "downclosed actions (sbMinus pre (sb pre))"
+     and downclosed_hb: "selective_downclosed ?f actions (release_acquire_fenced_hb pre wit)"
+  have final_sw: "\<And>x y. \<lbrakk>x \<in> actions; y \<in> actions; (x, y) \<in> ?sw\<rbrakk> \<Longrightarrow> (x, y) \<in> ?sw2"
+    using final_release_acquire_fenced_sw[OF downclosed_rf downclosed_mo downclosed_sb]
+    by metis 
+  show "selective_prefixes_are_final (is_na_or_non_write pre) 
+                                     actions 
+                                     (release_acquire_fenced_hb pre wit) 
+                                     (release_acquire_fenced_hb (preRestrict pre actions) (incWitRestrict wit actions))"
+    using final_no_consume_hb[OF downclosed_rf downclosed_mo] downclosed_hb final_sw
+    unfolding release_acquire_fenced_hb_def
+    by auto
+qed
+
+(* Prefixes are final in the with-consume fragment *)
+
+lemma final_cad:
+  assumes downclosed_sb: "\<And>a. (a, b) \<in> sb pre \<Longrightarrow> a \<in> actions"
+      and trans_sb:      "trans (sb pre)"
+      and dd_in_sb:      "dd pre \<subseteq> sb pre"
+      and b:             "b \<in> actions" 
+      and cad:           "(a, b) \<in> with_consume_cad_set_alt pre wit"
+  shows   "a \<in> actions \<and> (a, b) \<in> with_consume_cad_set_alt (preRestrict pre actions) (incWitRestrict wit actions)"
+proof -
+  have downclosed_cad: "\<And>c. (c, b) \<in> (rf wit \<inter> sb pre \<union> dd pre)\<^sup>+ \<Longrightarrow> c \<in> actions"
+    proof -
+      fix c
+      assume c: "(c, b) \<in> (rf wit \<inter> sb pre \<union> dd pre)\<^sup>+"
+      have "rf wit \<inter> sb pre \<union> dd pre \<subseteq> sb pre"
+        using `dd pre \<subseteq> sb pre` by auto
+      hence "(rf wit \<inter> sb pre \<union> dd pre)\<^sup>+ \<subseteq> sb pre"
+        using trancl_mono3[OF `trans (sb pre)`] by auto
+      hence "(c, b) \<in> sb pre" using c by auto
+      thus "c \<in> actions"
+        using downclosed_sb b unfolding downclosed_def by auto
+    qed
+  hence "a \<in> actions" 
+    using cad unfolding with_consume_cad_set_alt_def with_consume_cad_set_def by auto
+  have "(a, b) \<in> with_consume_cad_set_alt (preRestrict pre actions) (incWitRestrict wit actions)"
+    using cad unfolding with_consume_cad_set_alt_def with_consume_cad_set_def
+    proof (rule converse_trancl_induct)
+      fix y
+      assume y: "(y, b) \<in> rf wit \<inter> sb pre \<union> dd pre"
+      hence "(y, b) \<in> (rf wit \<inter> sb pre \<union> dd pre)\<^sup>+" by fast
+      hence "y \<in> actions" using downclosed_cad by fast
+      hence "(y, b) \<in> relRestrict (rf wit) actions \<inter> relRestrict (sb pre) actions \<union> relRestrict (dd pre) actions"
+        using y b by auto
+      thus "(y, b) \<in> (rf (incWitRestrict wit actions) \<inter> sb (preRestrict pre actions) \<union> dd (preRestrict pre actions))\<^sup>+" 
+        by auto
+    next
+      fix y z
+      assume y:  "(y, z) \<in> rf wit \<inter> sb pre \<union> dd pre"
+         and z:  "(z, b) \<in> (rf wit \<inter> sb pre \<union> dd pre)\<^sup>+"
+         and ih: "(z, b) \<in> (rf (incWitRestrict wit actions) \<inter> sb (preRestrict pre actions) \<union> dd (preRestrict pre actions))\<^sup>+"
+      have "z \<in> actions" using downclosed_cad[OF z] .
+      have "(y, b) \<in> (rf wit \<inter> sb pre \<union> dd pre)\<^sup>+" 
+        using y z by (rule trancl_into_trancl2)
+      hence "y \<in> actions" using downclosed_cad by fast
+      have "(y, z) \<in> relRestrict (rf wit) actions \<inter> relRestrict (sb pre) actions \<union> relRestrict (dd pre) actions"
+        using y `y \<in> actions` `z \<in> actions` by auto
+      thus "(y, b) \<in> (rf (incWitRestrict wit actions) \<inter> sb (preRestrict pre actions) \<union> dd (preRestrict pre actions))\<^sup>+"
+        using ih by (auto simp add: trancl_into_trancl2)
+    qed
+  thus ?thesis using `a \<in> actions` by simp
+qed
+
+lemma final_dob:
+  assumes downclosed_sb: "\<And>a. (a, d) \<in> sb pre \<Longrightarrow> a \<in> actions"
+      and downclosed_rf: "downclosed actions (rf wit)"
+      and downclosed_mo: "downclosed actions (mo wit)"
+      and trans_sb:      "trans (sb pre)"
+      and dd_in_sb:      "dd pre \<subseteq> sb pre"
+      and d:             "d \<in> actions" 
+      and dob_set:       "(a, d) \<in> with_consume_dob_set_alt pre wit"
+  shows   "(a, d) \<in> with_consume_dob_set_alt (preRestrict pre actions) (incWitRestrict wit actions)"
+proof -
+  obtain c b where a:  "a \<in> actions0 pre" "is_release a"
+               and rs: "(a, b) \<in> release_sequence_set_alt pre wit"
+               and b:  "b \<in> actions0 pre"
+               and rf: "(b, c) \<in> rf wit"
+               and c:  "c \<in> actions0 pre" "is_consume c"
+               and cad_or_eq: "(c, d) \<in> with_consume_cad_set_alt pre wit \<or> c = d"
+               and d2: "d \<in> actions0 pre"
+    using dob_set
+    unfolding with_consume_dob_set_alt_def 
+              with_consume_dob_set_def
+    by (auto simp add: dependency_ordered_before_def)
+  have cad2: "  (    (c, d) \<in> with_consume_cad_set_alt (preRestrict pre actions) (incWitRestrict wit actions) 
+                  \<or> (c = d))
+              \<and> c \<in> actions"
+    using cad_or_eq
+    proof
+      assume "c = d"
+      thus ?thesis using `d \<in> actions` by simp
+    next
+      assume "(c, d) \<in> with_consume_cad_set_alt pre wit"
+      thus ?thesis
+        using final_cad[OF downclosed_sb trans_sb dd_in_sb d]
+        by fast
+    qed
+  hence "b \<in> actions"
+    using rf downclosed_rf unfolding downclosed_def by fast
+  hence rf2: "(b, c) \<in> relRestrict (rf wit) actions" 
+    using cad2 rf by auto
+  have rs2: "  a \<in> actions 
+             \<and> (a, b) \<in> release_sequence_set_alt (preRestrict pre actions) (incWitRestrict wit actions)" 
+    using rs final_release_sequence[OF downclosed_mo `b \<in> actions`]
+    by fast
+  thus ?thesis
+    using a c d d2 b rs2 rf2 cad2
+    unfolding with_consume_dob_set_alt_def with_consume_dob_set_def
+    by (auto simp add: dependency_ordered_before_def)
+qed
+
+lemma UnMember_mono:
+  assumes "x \<in> s \<union> r"
+      and "x \<in> s \<Longrightarrow> x \<in> s'"
+      and "x \<in> r \<Longrightarrow> x \<in> r'"
+  shows   "x \<in> s' \<union> r'"
+using assms
+by auto
+
+lemma composeMember_mono:
+  assumes "(a, c) \<in> s O r"
+      and "\<And>b. (a, b) \<in> s \<Longrightarrow> (b, c) \<in> r \<Longrightarrow> (a, b) \<in> s' \<and> (b, c) \<in> r'"
+  shows   "(a, c) \<in> s' O r'"
+using assms
+by auto
+
+lemma final_ithb_r:
+  assumes downclosed_sb:  "\<And>a. (a, b) \<in> sb pre \<Longrightarrow> a \<in> actions"
+      and downclosed_sb2: "downclosed actions (sbMinus pre (sb pre))"
+      and downclosed_rf:  "downclosed actions (rf wit)"
+      and downclosed_mo:  "downclosed actions (mo wit)"
+      and trans_sb:       "trans (sb pre)"
+      and dd_in_sb:       "dd pre \<subseteq> sb pre"
+      and a:              "a \<in> actions" 
+      and b:              "b \<in> actions" 
+      and ithb:           "(a, b) \<in> inter_thread_happens_before_r pre wit"
+  shows   "(a, b) \<in> inter_thread_happens_before_r (preRestrict pre actions) (incWitRestrict wit actions)"
+using ithb
+unfolding inter_thread_happens_before_r_def
+apply (elim UnMember_mono)
+defer defer
+apply (simp, elim composeMember_mono)
+proof simp
+  assume "(a, b) \<in> with_consume_dob_set_alt pre wit"
+  thus "(a, b) \<in> with_consume_dob_set_alt (preRestrict pre actions) (incWitRestrict wit actions)"
+    using final_dob[OF downclosed_sb downclosed_rf downclosed_mo trans_sb dd_in_sb b]
+    by auto
+next
+  assume "(a, b) \<in> release_acquire_fenced_synchronizes_with_set_alt pre wit"
+  thus "(a, b) \<in> release_acquire_fenced_synchronizes_with_set_alt (preRestrict pre actions) (incWitRestrict wit actions)"
+    using final_release_acquire_fenced_sw[OF downclosed_rf downclosed_mo downclosed_sb2 a b]
+    by metis
+next
+  fix y
+  assume sw: "(a, y) \<in> release_acquire_fenced_synchronizes_with_set_alt pre wit"
+     and sb: "(y, b) \<in> sb pre"
+  have "y \<in> actions"
+    using sb downclosed_sb by auto
+  thus "(a, y) \<in> release_acquire_fenced_synchronizes_with_set_alt (preRestrict pre actions) (incWitRestrict wit actions)
+         \<and> y \<in> actions \<and> b \<in> actions"
+    using sw sb `b \<in> actions`
+    using final_release_acquire_fenced_sw[OF downclosed_rf downclosed_mo downclosed_sb2 a]
+    by metis
+qed
+
+lemma final_ithb_step:
+  assumes downclosed_sb:  "\<And>a. (a, b) \<in> sb pre \<Longrightarrow> a \<in> actions"
+      and downclosed_sb2: "downclosed actions (sbMinus pre (sb pre))"
+      and downclosed_rf:  "downclosed actions (rf wit)"
+      and downclosed_mo:  "downclosed actions (mo wit)"
+      and downclosed_ithb: "\<And>x.     (x, b) \<in> inter_thread_happens_before_alt pre wit
+                                 \<Longrightarrow> x \<in> actions"
+      and trans_sb:       "trans (sb pre)"
+      and dd_in_sb:       "dd pre \<subseteq> sb pre"
+      and a:              "a \<in> actions" 
+      and b:              "b \<in> actions" 
+      and ithb:           "(a, b) \<in> inter_thread_happens_before_step pre wit"
+  shows   "(a, b) \<in> inter_thread_happens_before_step (preRestrict pre actions) (incWitRestrict wit actions)"
+using ithb
+unfolding inter_thread_happens_before_step_def
+apply (elim UnMember_mono)
+defer 
+apply (simp, elim composeMember_mono)
+proof simp
+  assume "(a, b) \<in> inter_thread_happens_before_r pre wit"
+  thus "(a, b) \<in> inter_thread_happens_before_r (preRestrict pre actions) (incWitRestrict wit actions)"
+    using final_ithb_r[OF downclosed_sb downclosed_sb2 downclosed_rf downclosed_mo
+                          trans_sb dd_in_sb a b]
+    by metis
+next
+  fix y
+  assume sb: "(a, y) \<in> sb pre"
+     and r:  "(y, b) \<in> inter_thread_happens_before_r pre wit"
+  hence "(y, b) \<in> inter_thread_happens_before_alt pre wit"
+    unfolding inter_thread_happens_before_step_def
+              inter_thread_happens_before_alt_def 
+    by auto
+  hence "y \<in> actions"
+    using downclosed_ithb by auto
+  thus "  a \<in> actions \<and> y \<in> actions
+        \<and> (y, b) \<in> inter_thread_happens_before_r (preRestrict pre actions) (incWitRestrict wit actions)"
+    using final_ithb_r[OF downclosed_sb downclosed_sb2 downclosed_rf downclosed_mo
+                          trans_sb dd_in_sb]
+    using r a b sb
+    by metis
+qed
+
+lemma final_ithb:
+  assumes downclosed_sb:  "\<And>a. (a, b) \<in> sb pre \<Longrightarrow> a \<in> actions"
+      and downclosed_sb2: "downclosed actions (sbMinus pre (sb pre))"
+      and downclosed_rf:  "downclosed actions (rf wit)"
+      and downclosed_mo:  "downclosed actions (mo wit)"
+      and downclosed_ithb: "\<And>x.     (x, b) \<in> inter_thread_happens_before_alt pre wit
+                                 \<Longrightarrow> x \<in> actions"
+      and trans_sb:       "trans (sb pre)"
+      and dd_in_sb:       "dd pre \<subseteq> sb pre"
+      and b:              "b \<in> actions" 
+      and ithb:           "(a, b) \<in> inter_thread_happens_before_alt pre wit"
+  shows   "(a, b) \<in> inter_thread_happens_before_alt (preRestrict pre actions) (incWitRestrict wit actions)"
+using ithb
+unfolding inter_thread_happens_before_alt_def
+proof (induct rule: converse_trancl_induct)
+  fix y
+  assume step: "(y, b) \<in> inter_thread_happens_before_step pre wit"
+  hence "y \<in> actions"
+    using downclosed_ithb
+    unfolding inter_thread_happens_before_alt_def
+    by auto
+  thus "(y, b) \<in> (inter_thread_happens_before_step (preRestrict pre actions) (incWitRestrict wit actions))\<^sup>+"
+    using final_ithb_step[OF downclosed_sb downclosed_sb2 downclosed_rf 
+                             downclosed_mo downclosed_ithb trans_sb dd_in_sb _ b step]
+    by auto
+next
+  fix y z
+  assume yz: "(y, z) \<in> inter_thread_happens_before_step pre wit"
+     and zb: "(z, b) \<in> (inter_thread_happens_before_step pre wit)\<^sup>+"
+     and ih: "(z, b) \<in> (inter_thread_happens_before_step (preRestrict pre actions) (incWitRestrict wit actions))\<^sup>+"
+  have z: "z \<in> actions"
+    using zb downclosed_ithb
+    unfolding inter_thread_happens_before_alt_def
+    by auto
+  have "(y, b) \<in> (inter_thread_happens_before_step pre wit)\<^sup>+"
+    using yz zb by auto
+  hence y: "y \<in> actions"
+    using downclosed_ithb
+    unfolding inter_thread_happens_before_alt_def
+    by auto
+  (* TODO: refactor the following. *)
+  have downclosed_sb1b: "\<And>x. (x, z) \<in> sb pre \<Longrightarrow> x \<in> actions"
+    proof -
+      fix x
+      assume sb: "(x, z) \<in> sb pre"
+      obtain w where zw: "(z, w) \<in> inter_thread_happens_before_step pre wit"
+                 and wb: "(w, b) \<in> (inter_thread_happens_before_step pre wit)\<^sup>*"
+        using zb tranclD[of z b] by auto
+      have "(x, w) \<in> compose0 (sb pre) (inter_thread_happens_before_r pre wit)"
+        using zw 
+        unfolding inter_thread_happens_before_step_def
+        proof
+          assume "(z, w) \<in> inter_thread_happens_before_r pre wit"
+          thus "(x, w) \<in> compose0 (sb pre) (inter_thread_happens_before_r pre wit)"
+            using sb by auto
+        next
+          assume "(z, w) \<in> compose0 (sb pre) (inter_thread_happens_before_r pre wit)"
+          then obtain v where zv: "(z, v) \<in> sb pre"
+                          and vw: "(v, w) \<in> inter_thread_happens_before_r pre wit"
+            by auto
+          have "(x, v) \<in> sb pre"
+            using sb zv trans_sb by (auto elim: transE)
+          thus "(x, w) \<in> compose0 (sb pre) (inter_thread_happens_before_r pre wit)"
+            using vw by auto
+        qed
+      hence "(x, w) \<in> inter_thread_happens_before_step pre wit"
+        unfolding inter_thread_happens_before_step_def by auto
+      hence "(x, b) \<in> inter_thread_happens_before_alt pre wit"
+        using wb unfolding inter_thread_happens_before_alt_def by auto
+      thus "x \<in> actions" using downclosed_ithb by auto
+    qed
+  (* TODO: and also refactor the following. *)
+  have downclosed_ithb2: "\<And>x. (x, z) \<in> inter_thread_happens_before_alt pre wit \<Longrightarrow> x \<in> actions"
+    proof -
+      fix x
+      assume "(x, z) \<in> inter_thread_happens_before_alt pre wit"
+      hence "(x, b) \<in> inter_thread_happens_before_alt pre wit"
+        using zb unfolding inter_thread_happens_before_alt_def by auto
+      thus "x \<in> actions" using downclosed_ithb by auto
+    qed
+  hence "(y, z) \<in> (inter_thread_happens_before_step (preRestrict pre actions) (incWitRestrict wit actions))\<^sup>+"
+    using final_ithb_step[OF downclosed_sb1b downclosed_sb2 downclosed_rf 
+                             downclosed_mo downclosed_ithb2 trans_sb dd_in_sb y z yz]
+    by auto
+  thus "(y, b) \<in> (inter_thread_happens_before_step (preRestrict pre actions) (incWitRestrict wit actions))\<^sup>+"
+    using ih by auto
+qed
+
+lemma final_with_consume_hb_aux:
+  assumes downclosed_sb:  "\<And>a. (a, b) \<in> sb pre \<Longrightarrow> a \<in> actions"
+      and downclosed_sb2: "downclosed actions (sbMinus pre (sb pre))"
+      and downclosed_rf:  "downclosed actions (rf wit)"
+      and downclosed_mo:  "downclosed actions (mo wit)"
+      and downclosed_ithb: "\<And>x.     (x, b) \<in> inter_thread_happens_before_alt pre wit
+                                 \<Longrightarrow> x \<in> actions"
+      and trans_sb:      "trans (sb pre)"
+      and dd_in_sb:      "dd pre \<subseteq> sb pre"
+      and b:             "b \<in> actions" 
+      and hb:            "(a, b) \<in> with_consume_hb pre wit"
+  shows   "(a, b) \<in> with_consume_hb (preRestrict pre actions) (incWitRestrict wit actions)"
+using hb
+unfolding with_consume_hb_def happens_before_def
+proof (rule UnMember_mono)
+  assume "(a, b) \<in> sb pre"
+  hence "a \<in> actions" using downclosed_sb by auto
+  thus "(a, b) \<in> sb (preRestrict pre actions)"
+    using `(a, b) \<in> sb pre` b by auto
+next
+  assume ithb: "(a, b) \<in> inter_thread_happens_before_alt pre wit"
+  show "(a, b) \<in> inter_thread_happens_before_alt (preRestrict pre actions) (incWitRestrict wit actions)"
+    using final_ithb[OF downclosed_sb downclosed_sb2 downclosed_rf downclosed_mo
+                        downclosed_ithb trans_sb dd_in_sb b(1) ithb]
+    by simp
+qed
+
+lemma final_with_consume_hb:
+  shows   "hbCalcIsFinalForPrefixes with_consume_hb"
+unfolding hbCalcIsFinalForPrefixes_def 
+proof auto
+  fix pre :: pre_execution
+  fix wit :: execution_witness
+  fix actions
+  let ?sw   = "release_acquire_fenced_synchronizes_with_set_alt pre wit"
+  let ?sw2  = "release_acquire_fenced_synchronizes_with_set_alt (preRestrict pre actions) (incWitRestrict wit actions)"
+  let ?f    = "is_na_or_non_write pre"
+  assume downclosed_rf: "downclosed actions (rf wit)" 
+     and downclosed_mo: "downclosed actions (mo wit)"
+     and downclosed_sb: "downclosed actions (sbMinus pre (sb pre))"
+     and downclosed_hb: "selective_downclosed ?f actions (with_consume_hb pre wit)"
+     and trans_sb:      "trans (sb pre)"
+     and dd_in_sb:      "dd pre \<subseteq> sb pre"
+  show "selective_prefixes_are_final (is_na_or_non_write pre) 
+                                     actions 
+                                     (with_consume_hb pre wit) 
+                                     (with_consume_hb (preRestrict pre actions) (incWitRestrict wit actions))"
+    unfolding selective_prefixes_are_final_def
+    (* TODO: remove redundancies *)
+    proof auto
+      fix a b
+      assume b:  "b \<in> actions" "is_na_or_non_write pre b"
+         and ab: "(a, b) \<in> with_consume_hb pre wit"
+      have downclosed_sb2:  "\<And>a. (a, b) \<in> sb pre \<Longrightarrow> a \<in> actions"
+        using downclosed_hb b
+        unfolding selective_downclosed_def 
+                  with_consume_hb_def 
+                  happens_before_def
+        by auto
+      have downclosed_ithb: "\<And>x. (x, b) \<in> inter_thread_happens_before_alt pre wit \<Longrightarrow> x \<in> actions" 
+        using downclosed_hb b
+        unfolding selective_downclosed_def 
+                  with_consume_hb_def 
+                  happens_before_def
+        by auto
+      show "(a, b) \<in> with_consume_hb (preRestrict pre actions) (incWitRestrict wit actions)"
+        using final_with_consume_hb_aux[OF downclosed_sb2 downclosed_sb downclosed_rf
+                                           downclosed_mo downclosed_ithb trans_sb
+                                           dd_in_sb b(1) ab]
+        by metis
+    qed
+qed
+
+subsubsection {* Summary *}
+
+(* The properties proven for the fragment used in the opsem *)
+
+lemma hbRelOver:
+  assumes "relOver (sb pre) (actions0 pre)"
+  shows   "relOver (getHb pre wit) (actions0 pre)"
+using relOver_with_consume_hb assms
+by auto
+
+lemma sbInHb:
+  shows "sb pre \<subseteq> getHb pre wit"
+using sbInHb_with_consume_hb
+by auto
+
+lemma loInHb:
+  shows "hbCalcRespectsSyncingLocks getHb"
+using loInHb_with_consume_hb 
+by auto
+
+lemma hbCalcIsMonotonic:
+  shows "hbCalcIsMonotonic getHb"
+using monotonicity_with_consume_hb 
+unfolding hbCalcIsMonotonic_def
+by auto
+
+lemma hbCalcIsFinalForPrefixes:
+  shows "hbCalcIsFinalForPrefixes getHb"
+using final_with_consume_hb 
+by auto
+
+(* Corollaries for derived relations *)
+
+lemma hbMinusIsMonotonic:
+  shows "hbCalcIsMonotonic hbMinusAlt"
+using hbCalcIsMonotonic
+(* TODO: make a simp for "hbMinus pre wit getRelations" to "hbMinus pre wit getHb". *)
+unfolding hbCalcIsMonotonic_def 
+          getRelations_simp 
+          hbMinusAlt_def
+by auto
+
+lemma opsemOrderIsMonotonic:
+  shows "hbCalcIsMonotonic incComAlt"
+unfolding hbCalcIsMonotonic_def
+proof (intro allI impI)
+  fix pre
+  fix wit :: execution_witness
+  fix actions
+  assume downclosed: "downclosed actions (mo wit)"
+  have "hbMinusAlt (preRestrict pre actions) (incWitRestrict wit actions) \<subseteq> hbMinusAlt pre wit"
+    using downclosed hbMinusIsMonotonic
+    unfolding hbCalcIsMonotonic_def by metis
+  hence subset: "hbMinusAlt (preRestrict pre actions) (incWitRestrict wit actions) \<union> 
+                (rf (incWitRestrict wit actions) \<union> 
+                 mo (incWitRestrict wit actions)) \<subseteq> 
+                hbMinusAlt pre wit \<union> (rf wit \<union> mo wit)" 
+    by auto
+  show "incComAlt (preRestrict pre actions) (incWitRestrict wit actions) \<subseteq> incComAlt pre wit"
+    unfolding incComAlt_def 
+    using subset trancl_mono2
+    by metis
+qed
+
+subsection {* Invariance of consistency predicates under prefixes *}
+
+lemma final_vse:
+  assumes final: "selective_prefixes_are_final f actions hb hb2"
+      and        "hb2 \<subseteq> hb"
+                 "f b"
+                 "b \<in> actions"
+      and vse:   "(a, b) \<in> visible_side_effect_set (actions0 pre) hb"
+  shows          "(a, b) \<in> visible_side_effect_set (actions0 pre) hb2"
+proof -
+  have as1: "\<not> (\<exists>c\<in>actions0 pre. c \<notin> {a, b} \<and> is_write c \<and> loc_of c = loc_of b \<and> (a, c) \<in> hb2 \<and> (c, b) \<in> hb2)"
+    using vse `hb2 \<subseteq> hb` unfolding visible_side_effect_set_def by auto
+  have as2: "(a, b) \<in> hb \<and> is_write a \<and> is_read b \<and> loc_of a = loc_of b"
+    using vse unfolding visible_side_effect_set_def by auto
+  hence "(a, b) \<in> hb2"
+    using final `f b` `b \<in> actions` unfolding selective_prefixes_are_final_def by auto
+  thus "(a, b) \<in> visible_side_effect_set (actions0 pre) hb2"
+    using as1 as2 unfolding visible_side_effect_set_def by auto
+qed
+
+lemma assumptions_restriction:
+  assumes "assumptions (pre, wit, [])"
+  shows   "assumptions (preRestrict pre actions, incWitRestrict wit actions, [])"
+using assms
+unfolding assumptions.simps finite_prefixes_def
+by auto
+
+lemma coherent_memory_use_restriction:
+  assumes "coherent_memory_use (pre, wit, [(''hb'', hb)])"
+          "hb2 \<subseteq> hb"
+  shows   "coherent_memory_use (preRestrict pre actions, incWitRestrict wit actions, [(''hb'', hb2)])"
+using assms
+unfolding coherent_memory_use.simps  
+by auto blast+ 
+
+lemma consistent_atomic_rf_restriction:
+  assumes "consistent_atomic_rf (pre, wit, [(''hb'', hb)])"
+          "hb2 \<subseteq> hb"
+  shows   "consistent_atomic_rf (preRestrict pre actions, incWitRestrict wit actions, [(''hb'', hb2)])"
+using assms
+unfolding consistent_atomic_rf.simps 
+by auto
+
+lemma consistent_hb_restriction:
+  assumes "consistent_hb (pre, wit, [(''hb'', hb)])"
+          "hb2 \<subseteq> hb"
+  shows   "consistent_hb (preRestrict pre actions, incWitRestrict wit actions, [(''hb'', hb2)])"
+using assms
+unfolding consistent_hb.simps 
+proof auto
+  assume "irrefl (hb\<^sup>+)" 
+     and "hb2 \<subseteq> hb"
+  hence "hb2\<^sup>+ \<subseteq> hb\<^sup>+" using trancl_mono2 by metis
+  thus "irrefl (hb2\<^sup>+)" using `irrefl (hb\<^sup>+)` 
+    unfolding irrefl_def by auto
+next
+  assume "finite_prefixes hb (actions0 pre)"
+     and "hb2 \<subseteq> hb"
+  thus "finite_prefixes hb2 (actions0 pre \<inter> actions)"
+    using finite_prefix_subset
+    by force
+qed
+
+lemma consistent_mo_restriction:
+  assumes "consistent_mo (pre, wit, [])"
+          "downclosed actions (mo wit)"
+  shows   "consistent_mo (preRestrict pre actions, incWitRestrict wit actions, [])"
+using assms
+unfolding consistent_mo.simps downclosed_def
+by auto
+
+lemma consistent_non_atomic_rf_restriction:
+  fixes pre wit hb hb2 actions
+  defines "vse  \<equiv>  visible_side_effect_set (actions0 pre) hb"
+      and "vse2 \<equiv>  visible_side_effect_set (actions0 (preRestrict pre actions)) hb2"
+  assumes cons_rf: "consistent_non_atomic_rf (pre, wit, [(''hb'', hb),(''vse'', vse)])"
+      and final:   "selective_prefixes_are_final (is_na_or_non_write pre) actions hb hb2"
+      and          "hb2 \<subseteq> hb"
+  shows   "consistent_non_atomic_rf (preRestrict pre actions, incWitRestrict wit actions, [(''hb'', hb2),(''vse'', vse2)])"
+unfolding consistent_non_atomic_rf.simps 
+proof auto
+  fix a b
+  assume loc: "is_at_non_atomic_location (lk pre) b"
+     and      "(a, b) \<in> rf wit"
+              "a \<in> actions" 
+              "b \<in> actions"
+  hence non_write_b: "is_na_or_non_write pre b"
+    unfolding is_na_or_non_write_def by simp
+  have vse: "(a, b) \<in> vse"
+    using cons_rf `(a, b) \<in> rf wit` loc unfolding consistent_non_atomic_rf.simps by auto
+  thus "(a, b) \<in> vse2"
+    using final_vse[OF final `hb2 \<subseteq> hb` non_write_b `b \<in> actions`, where a=a] 
+    using `a \<in> actions` `b \<in> actions`
+    unfolding vse_def vse2_def visible_side_effect_set_def by auto
+qed
+
+lemma det_read_alt_restriction:
+  assumes det_read:      "det_read_alt (pre, wit, [(''hb'', hb)])"
+      and conshb:        "consistent_hb (pre, wit, [(''hb'', hb)])"
+      and downclosed_rf: "downclosed actions (rf wit)"
+      and downclosed_hb: "downclosed actions (hbMinus (pre, wit, [(''hb'', hb)]))"
+      and final:         "selective_prefixes_are_final (is_na_or_non_write pre) actions hb hb2"
+      and                "hb2 \<subseteq> hb"
+  shows   "det_read_alt (preRestrict pre actions, incWitRestrict wit actions, [(''hb'', hb2)])"
+unfolding det_read_alt.simps
+proof (clarsimp)
+  fix r 
+  assume "r \<in> actions0 pre" 
+         "is_load r"
+         "r \<in> actions"
+  hence non_write_r: "is_na_or_non_write pre r"
+    unfolding is_na_or_non_write_def by (cases r) auto
+  hence hb_eq: "\<And>w. ((w, r) \<in> hb2) = ((w, r) \<in> hb)"
+    using `hb2 \<subseteq> hb` final `r \<in> actions`
+    unfolding selective_prefixes_are_final_def 
+    by auto  
+  show "  (\<exists>w\<in>actions0 pre \<inter> actions. (w, r) \<in> hb2 \<and> is_write w \<and> loc_of w = loc_of r)  
+        = (\<exists>w'\<in>actions0 pre \<inter> actions. (w', r) \<in> rf wit)"
+    proof auto
+      fix w
+      assume w: "w \<in> actions0 pre"
+                "w \<in> actions"
+                "(w, r) \<in> hb2"
+                "is_write w"
+                "loc_of w = loc_of r"
+      hence "(w, r) \<in> hb" using hb_eq by auto
+      then obtain w' where w': "w'\<in>actions0 pre" "(w', r) \<in> rf wit"
+        using w det_read `is_load r` `r \<in> actions0 pre`
+        unfolding det_read_alt.simps 
+        by auto
+      hence "w' \<in> actions"
+        using downclosed_rf `r \<in> actions` unfolding downclosed_def by auto
+      thus "\<exists>w'\<in>actions0 pre \<inter> actions. (w', r) \<in> rf wit"
+        using w' by auto
+    next
+      fix w'
+      assume w': "(w', r) \<in> rf wit"
+                 "w' \<in> actions0 pre"
+                 "w' \<in> actions"
+      then obtain w where w: "w \<in> actions0 pre"
+                              "(w, r) \<in> hb"
+                              "is_write w"
+                              "loc_of w = loc_of r"
+        using w' det_read `is_load r` `r \<in> actions0 pre`
+        unfolding det_read_alt.simps 
+        by auto
+      hence "w \<in> actions"
+        using non_write_r downclosed_hb `r \<in> actions`
+        unfolding hbMinus.simps downclosed_def
+        by auto
+      have "(w, r) \<in> hb2" using `(w, r) \<in> hb` hb_eq by auto
+      thus "\<exists>w\<in>actions0 pre \<inter> actions. (w, r) \<in> hb2 \<and> is_write w \<and> loc_of w = loc_of r"
+        using w `w \<in> actions` by auto
+    qed
+(*
+  hence "  (\<exists>w\<in>actions0 pre \<inter> actions. (w, r) \<in> hb2 \<and> is_write w \<and> loc_of w = loc_of r)
+         = (\<exists>w\<in>actions0 pre \<inter> actions. (w, r) \<in> hb \<and> is_write w \<and> loc_of w = loc_of r)"
+    by auto
+  also have "... = (\<exists>w'\<in>actions0 pre \<inter> actions. (w', r) \<in> rf wit)"
+    using det_read `is_load r` `r \<in> actions0 pre` downclosed_rf downclosed_hb non_write_r
+    unfolding det_read_alt.simps downclosed_def hbMinus.simps
+    by auto
+  also have "... = (\<exists>w'\<in>actions0 pre \<inter> actions. (w', r) \<in> rf wit)"
+    using downclosed_rf `r \<in> actions` unfolding downclosed_def by auto
+  finally show "  (\<exists>w\<in>actions0 pre \<inter> actions. (w, r) \<in> hb2 \<and> is_write w \<and> loc_of w = loc_of r)  
+                = (\<exists>w'\<in>actions0 pre \<inter> actions. (w', r) \<in> rf wit)" .
+*)
+qed
+
+lemma locks_only_consistent_lo_restriction:
+  assumes "locks_only_consistent_lo (pre, wit, [(''hb'', hb)])"
+          "hb2 \<subseteq> hb"
+  shows   "locks_only_consistent_lo (preRestrict pre actions, incWitRestrict wit actions, [(''hb'', hb2)])"
+proof -
+  obtain hb3 where [simp]: "hb = hb2 \<union> hb3" using `hb2 \<subseteq> hb` by auto
+  show ?thesis 
+    using assms relRestrict_relOver relRestrict_isTransitive relRestrict_isIrreflexive
+    unfolding locks_only_consistent_lo.simps 
+    by auto
+qed
+
+lemma locks_only_consistent_locks_restriction:
+  assumes "locks_only_consistent_locks (pre, wit, [])"
+          "selective_downclosed (is_na_or_non_write pre) actions (getHb pre wit)"
+          "\<And>a b. \<lbrakk>is_unlock a; is_lock b; (a, b) \<in> lo wit\<rbrakk> \<Longrightarrow> (a, b) \<in> getHb pre wit"
+  shows   "locks_only_consistent_locks (preRestrict pre actions, incWitRestrict wit actions, [])"
+unfolding locks_only_consistent_locks.simps
+proof auto
+  fix a b
+  assume assms2: "is_successful_lock a"
+                 "is_successful_lock b"
+                 "a \<in> actions"
+                 "b \<in> actions"
+                 "(a, b) \<in> lo wit"
+  hence "is_lock b" by (cases b) auto
+  have "is_na_or_non_write pre b" using assms2 unfolding is_na_or_non_write_def by (cases b) auto
+  obtain c where assms3: "c \<in> actions0 pre \<and> is_unlock c \<and> (a, c) \<in> lo wit \<and> (c, b) \<in> lo wit"
+    using assms assms2 unfolding locks_only_consistent_locks.simps by blast
+  hence "(c, b) \<in> getHb pre wit"
+    using assms `is_lock b` by metis
+  hence "c \<in> actions" 
+    using assms assms2 `is_na_or_non_write pre b` `b \<in> actions`
+    unfolding selective_downclosed_def by auto
+  thus "\<exists>c\<in>actions0 pre \<inter> actions. is_unlock c \<and> (a, c) \<in> lo wit \<and> (c, b) \<in> lo wit"
+    using assms3 by fast
+qed
+
+lemma rmw_atomicity_restriction:
+  assumes "rmw_atomicity (pre, wit, [])"
+          "downclosed actions (mo wit)"
+  shows   "rmw_atomicity (preRestrict pre actions, incWitRestrict wit actions, [])"
+using assms
+unfolding rmw_atomicity.simps
+          adjacent_less_than_def
+          downclosed_def
+by auto
+
+lemma sc_accesses_consistent_sc_restriction:
+  assumes "sc_accesses_consistent_sc (pre, wit, [(''hb'', hb)])"
+          "hb2 \<subseteq> hb"
+  shows   "sc_accesses_consistent_sc (preRestrict pre actions, incWitRestrict wit actions, [(''hb'', hb2)])"
+proof -
+  obtain hb3 where [simp]: "hb = hb2 \<union> hb3" using `hb2 \<subseteq> hb` by auto
+  show ?thesis 
+    using assms relRestrict_relOver relRestrict_isTransitive relRestrict_isIrreflexive
+    unfolding sc_accesses_consistent_sc.simps
+    by auto
+qed
+
+lemma sc_accesses_sc_reads_restricted_restriction:
+  assumes "sc_accesses_sc_reads_restricted (pre, wit, [(''hb'', hb)])"
+          "hb2 \<subseteq> hb"
+  shows   "sc_accesses_sc_reads_restricted (preRestrict pre actions, incWitRestrict wit actions, [(''hb'', hb2)])"
+proof -
+  obtain hb3 where [simp]: "hb = hb2 \<union> hb3" using `hb2 \<subseteq> hb` by auto
+  show ?thesis 
+    using assms
+    unfolding sc_accesses_sc_reads_restricted.simps 
+    by auto
+qed
+
+lemma sc_fenced_sc_fences_heeded_restriction:
+  assumes "sc_fenced_sc_fences_heeded (pre, wit, [])"
+  shows   "sc_fenced_sc_fences_heeded (preRestrict pre actions, incWitRestrict wit actions, [])"
+using assms
+unfolding sc_fenced_sc_fences_heeded.simps 
+(* The simp takes a long time, but it is a difficult predicate. *)
+apply simp
+by auto
+
+lemma tot_empty_restriction:
+  assumes "tot_empty (pre, wit, [])"
+  shows   "tot_empty (preRestrict pre actions, incWitRestrict wit actions, [])"
+using assms
+unfolding tot_empty.simps 
+by simp
+
+lemma well_formed_rf_restriction:
+  assumes "well_formed_rf (pre, wit, [])"
+  shows   "well_formed_rf (preRestrict pre actions, incWitRestrict wit actions, [])"
+using assms
+unfolding well_formed_rf.simps 
+(* Without the clarsimp, auto takes a long, long time. *)
+by clarsimp auto
+
+lemma well_formed_threads_restriction:
+  assumes "well_formed_threads (pre, wit, [])"
+  shows   "well_formed_threads (preRestrict pre actions, wit2, [])"
+proof -
+  have "actions_respect_location_kinds (actions0 pre \<inter> actions) (lk pre)"
+    using assms
+    unfolding well_formed_threads.simps actions_respect_location_kinds_def
+    by auto
+  moreover have "irrefl (sbasw (preRestrict pre actions))"
+    using assms isIrreflexive_subset[OF _ incPreRestrict_sbasw_subset2]
+    unfolding well_formed_threads.simps 
+    by simp
+  moreover have "finite_prefixes (sbasw (preRestrict pre actions)) (actions0 pre \<inter> actions)"
+    using assms  finite_prefix_subset[OF _ incPreRestrict_sbasw_subset2]
+    unfolding well_formed_threads.simps
+    by auto
+  ultimately show ?thesis
+    using assms incPreRestrict_sbasw_subset
+    unfolding well_formed_threads.simps
+    unfolding blocking_observed_def
+              Cmm_master.inj_on_def
+              threadwise_def
+              interthread_def
+              isStrictPartialOrder_def
+              indeterminate_sequencing_def
+              disjoint_allocs_def
+    by auto
+qed
+
+lemma well_formed_threads_opsem_restriction:
+  assumes "well_formed_threads_opsem (pre, wit, [])"
+  shows   "well_formed_threads_opsem (preRestrict pre actions, wit2, [])"
+using assms
+unfolding well_formed_threads_opsem_eq
+using well_formed_threads_restriction
+by auto
+
+lemma axsimpConsistent_restriction:
+  assumes cons:       "axsimpConsistentAlt pre wit"
+      and downclosed: "downclosed actions (incComAlt pre wit)"
+  shows   "axsimpConsistentAlt (preRestrict pre actions) (incWitRestrict wit actions)"
+proof -
+  let ?wit' = "incWitRestrict wit actions"
+  let ?pre' = "preRestrict pre actions"
+  have downclosed_hbMinus: "downclosed actions (hbMinusAlt pre wit)"
+   and downclosed_rf:      "downclosed actions (rf wit)"
+   and downclosed_mo:      "downclosed actions (mo wit)"
+    using downclosed unfolding incComAlt_def by simp_all
+  have "sbMinus pre (sb pre) \<subseteq> hbMinusAlt pre wit" 
+    using sbInHb unfolding sbMinus_def getRelations_simp hbMinus.simps by auto
+  hence downclosed_sbMinus: "downclosed actions (sbMinus pre (sb pre))"
+    using downclosed_hbMinus downclosed_subset by metis
+  have selective_downclosed: "selective_downclosed (is_na_or_non_write pre) actions (getHb pre wit)"
+    using downclosed_hbMinus
+    unfolding getRelations_simp
+              hbMinus.simps
+              selective_downclosed_def
+              downclosed_def
+    by auto
+  have trans_sb: "trans (sb pre)"
+    using cons
+    by auto
+  have dd_subset_sb: "dd pre \<subseteq> sb pre"
+    using cons
+    by auto
+  have prefixes_final: "selective_prefixes_are_final (is_na_or_non_write pre) actions (getHb pre wit) (getHb ?pre' ?wit')"
+    using hbCalcIsFinalForPrefixes downclosed_rf downclosed_mo 
+          downclosed_sbMinus selective_downclosed trans_sb dd_subset_sb
+    unfolding hbCalcIsFinalForPrefixes_def hbMinus_def 
+    by auto
+
+  have hbSubset: "getHb ?pre' ?wit' \<subseteq> getHb pre wit"
+    using hbCalcIsMonotonic downclosed_mo unfolding hbCalcIsMonotonic_def by auto
+  
+  show ?thesis
+    unfolding axsimpConsistent_def
+    proof auto
+      show "assumptions (?pre', ?wit', [])"
+        using cons assumptions_restriction by auto
+    next
+      show "det_read_alt (?pre', ?wit', [(''hb'', getHb ?pre' ?wit')])"
+        using cons det_read_alt_restriction[OF _ _ downclosed_rf _ prefixes_final hbSubset]
+        using downclosed_hbMinus
+        by auto
+    next
+      show "coherent_memory_use (?pre', ?wit', [(''hb'', getHb ?pre' ?wit')])"
+        using cons coherent_memory_use_restriction hbSubset 
+        by auto
+    next
+      show "consistent_atomic_rf (?pre', ?wit', [(''hb'', getHb ?pre' ?wit')])"
+        using cons consistent_atomic_rf_restriction hbSubset 
+        by auto
+    next
+      show "consistent_hb (?pre', ?wit', [(''hb'', getHb ?pre' ?wit')])"
+        using cons consistent_hb_restriction hbSubset 
+        by auto
+    next
+      show "consistent_mo (?pre', ?wit', [])"
+        using cons consistent_mo_restriction downclosed_mo
+        by auto
+    next
+      have "consistent_non_atomic_rf (pre, wit, [(''hb'', getHb pre wit), (''vse'', getVse pre wit)])"
+        using cons by auto
+      thus "consistent_non_atomic_rf (?pre', ?wit', [(''hb'', getHb ?pre' ?wit'), (''vse'', getVse ?pre' ?wit')])"
+        using consistent_non_atomic_rf_restriction[OF _ prefixes_final hbSubset, where wit=wit]
+        unfolding getVse_def
+        by auto
+    next
+      show "locks_only_consistent_lo (?pre', ?wit', [(''hb'', getHb ?pre' ?wit')])"
+        using cons locks_only_consistent_lo_restriction hbSubset 
+        by auto
+    next
+      have "\<And>a b. is_unlock a \<Longrightarrow> is_lock b \<Longrightarrow> (a, b) \<in> lo wit \<Longrightarrow> (a, b) \<in> getHb pre wit"
+        using loInHb cons 
+        unfolding hbCalcRespectsSyncingLocks_def
+        by auto
+      thus "locks_only_consistent_locks (?pre', ?wit', [])"
+        using locks_only_consistent_locks_restriction[where pre=pre and wit=wit and actions=actions]
+        using selective_downclosed cons 
+        by auto
+    next
+      show "rmw_atomicity (?pre', ?wit', [])"
+        using cons rmw_atomicity_restriction downclosed_mo by auto
+    next
+      show "sc_accesses_consistent_sc (?pre', ?wit', [(''hb'', getHb ?pre' ?wit')])"
+        using cons sc_accesses_consistent_sc_restriction hbSubset by auto
+    next
+      show "sc_accesses_sc_reads_restricted (?pre', ?wit', [(''hb'', getHb ?pre' ?wit')])"
+        using cons sc_accesses_sc_reads_restricted_restriction hbSubset by auto
+    next
+      show "sc_fenced_sc_fences_heeded (?pre', ?wit', [])"
+        using cons sc_fenced_sc_fences_heeded_restriction by auto
+    next
+      show "tot_empty (?pre', ?wit', [])"
+        using cons tot_empty_restriction by auto
+    next
+      show "well_formed_rf (?pre', ?wit', [])"
+        using cons well_formed_rf_restriction by auto
+    next
+      show "well_formed_threads_opsem (?pre', ?wit', [])"
+        using cons well_formed_threads_opsem_restriction by auto
+    qed
+qed
+
+subsection {* Soundness *}
+
+(* Consistency of empty_witness *)
+
+lemma assumptions_empty_witness [simp]:
+  shows "assumptions ((preRestrict pre {}), empty_witness, [])"
+unfolding assumptions.simps
+by simp
+
+lemma well_formed_threads_empty_witness [simp]:
+  shows "well_formed_threads ((preRestrict pre {}), empty_witness, [])"
+unfolding well_formed_threads.simps indeterminate_sequencing_def
+by simp
+
+lemma well_formed_threads_opsem_empty_witness [simp]:
+  shows "well_formed_threads_opsem ((preRestrict pre {}), empty_witness, [])"
+unfolding well_formed_threads_opsem_eq
+by simp
+
+lemma det_read_op_empty_witness [simp]:
+  shows "det_read_alt ((preRestrict pre {}), empty_witness, [(''hb'', {})])"
+unfolding det_read_alt.simps
+by simp
+
+lemma coherent_memory_use_empty_witness [simp]:
+  shows "coherent_memory_use ((preRestrict pre {}), empty_witness, [(''hb'', {})])"
+unfolding coherent_memory_use.simps
+by simp
+
+lemma consistent_atomic_rf_empty_witness [simp]:
+  shows "consistent_atomic_rf ((preRestrict pre {}), empty_witness, [(''hb'', {})])"
+unfolding consistent_atomic_rf.simps
+by simp
+
+lemma consistent_mo_op_empty_witness [simp]:
+  shows "consistent_mo ((preRestrict pre {}), empty_witness, [])"
+unfolding consistent_mo.simps
+by simp
+
+lemma consistent_hb_empty_witness [simp]:
+  shows "consistent_hb ((preRestrict pre {}), empty_witness, [(''hb'', {})])"
+unfolding consistent_hb.simps 
+by simp
+
+lemma consistent_non_atomic_rf_empty_witness [simp]:
+  shows "consistent_non_atomic_rf ((preRestrict pre {}), empty_witness, [(''hb'', {}), (''vse'', {})])"
+unfolding consistent_non_atomic_rf.simps
+by simp
+
+lemma locks_only_consistent_lo_op_empty_witness [simp]:
+  shows "locks_only_consistent_lo ((preRestrict pre {}), empty_witness, [(''hb'', {})])"
+unfolding locks_only_consistent_lo.simps 
+by simp
+
+lemma locks_only_consistent_locks_op_empty_witness [simp]:
+  shows "locks_only_consistent_locks ((preRestrict pre {}), empty_witness, [])"
+unfolding locks_only_consistent_locks.simps
+by simp
+
+lemma rmw_atomicity_op_empty_witness [simp]:
+  shows "rmw_atomicity ((preRestrict pre {}), empty_witness, [])"
+unfolding rmw_atomicity.simps
+by simp
+
+lemma sc_accesses_consistent_sc_op_empty_witness [simp]:
+  shows "sc_accesses_consistent_sc ((preRestrict pre {}), empty_witness, [(''hb'', {})])"
+unfolding sc_accesses_consistent_sc.simps 
+by simp
+
+lemma sc_accesses_sc_reads_restricted_empty_witness [simp]:
+  shows "sc_accesses_sc_reads_restricted ((preRestrict pre {}), empty_witness, [(''hb'', {})])"
+unfolding sc_accesses_sc_reads_restricted.simps
+by simp
+
+lemma sc_fenced_sc_fences_heeded_empty_witness [simp]:
+  shows "sc_fenced_sc_fences_heeded ((preRestrict pre {}), empty_witness, [])"
+unfolding sc_fenced_sc_fences_heeded.simps
+by simp
+
+lemma tot_empty_empty_witness [simp]:
+  shows "tot_empty ((preRestrict pre {}), empty_witness, [])"
+unfolding tot_empty.simps
+by simp
+
+lemma well_formed_rf_op_empty_witness [simp]:
+  shows "well_formed_rf ((preRestrict pre {}), empty_witness, [])"
+unfolding well_formed_rf.simps
+by simp
+
+lemma consistencyEmptyExecution [simp]:
+  shows "axsimpConsistentAlt (preRestrict pre {}) empty_witness"
+unfolding axsimpConsistentAlt_def
+by simp
+
+lemma incTraceConsistency: 
+  assumes "incTrace pre r s"
+          "r = incInitialState pre"
+  shows   "  axsimpConsistentAlt (preRestrict pre (incCommitted s)) (incWit s)
+           \<and> well_formed_threads_opsem (pre, empty_witness, [])"
+using assms 
+proof induct
+  case incStep
+  thus ?case unfolding incStep_def Let_def by auto
+qed simp
+
+lemma incConsistentSoundness:
+  assumes "incConsistent (pre, wit, getRelations pre wit)"
+  shows   "axsimpConsistent (pre, wit, getRelations pre wit)"
+using assms
+proof -
+  assume "incConsistent (pre, wit, getRelations pre wit)"
+  then obtain s where trace: "incTrace pre (incInitialState pre) s"
+                  and   wit: "incWit s = wit"
+                  and   com: "incCommitted s = actions0 pre"
+    unfolding incConsistent.simps by auto
+  thus "axsimpConsistent (pre, wit, getRelations pre wit)" 
+    using incTraceConsistency[OF trace] preRestrict_id wit
+    by metis
+qed
+
+subsection {* Completeness *}
+
+lemma existenceIncTrace:
+  assumes cons:       "axsimpConsistentAlt pre wit"
+      and finite:     "finite actions"
+      and universe:   "actions \<subseteq> actions0 pre"
+      and downclosed: "downclosed actions (incComAlt pre wit)"
+  shows   "\<exists> s. incTrace pre (incInitialState pre) s \<and> 
+                incWit s = incWitRestrict wit actions \<and> 
+                incCommitted s = actions"
+proof (rule finite_downclosedsubset_induct[where R="(incComAlt pre wit)" and B="actions0 pre"])
+  show "finite actions" using finite .
+next
+  show "actions \<subseteq> actions0 pre" using universe .
+next
+  show "downclosed actions (incComAlt pre wit)" using downclosed .
+next
+  show "acyclic (incComAlt pre wit)"
+    using opsemOrder_isStrictPartialOrder[OF cons]
+    unfolding isStrictPartialOrder_def acyclic_def irrefl_def
+    by auto
+next
+  have "well_formed_threads_opsem (pre, wit, [])"
+    using cons by auto
+  hence "well_formed_threads_opsem (pre, empty_witness, [])"
+    by (cases "wit = empty_witness") simp_all
+  thus "\<exists>s.   incTrace pre (incInitialState pre) s 
+            \<and> incWit s = incWitRestrict wit {} 
+            \<and> incCommitted s = {}"
+    using incReflexive by (intro exI[where x="incInitialState pre"]) simp
+next
+  fix a :: action
+  fix actions :: "action set"
+  assume finite':     "finite actions"
+     and              "a \<notin> actions"
+     and              "a \<in> actions0 pre"
+     and downclosed': "downclosed (insert a actions) (incComAlt pre wit)"
+     and max:         "\<forall>b\<in>actions. (a, b) \<notin> incComAlt pre wit"
+     and IH:          "\<exists>s. incTrace pre (incInitialState pre) s \<and> 
+                           incWit s = incWitRestrict wit actions \<and> 
+                           incCommitted s = actions"
+  obtain s where trace:     "incTrace pre (incInitialState pre) s" 
+             and witness:   "incWit s = incWitRestrict wit actions"
+             and committed: "incCommitted s = actions" using IH by blast
+
+  let ?actions' = "insert a actions"
+  let ?pre'     = "preRestrict pre ?actions'"
+  let ?wit'     = "incWitRestrict wit ?actions'"
+  let ?s' = "\<lparr> incWit=?wit', 
+               incCommitted=?actions'\<rparr>"
+  have downclosed_mo: "downclosed ?actions' (mo wit)"
+    using downclosed' unfolding incComAlt_def by auto
+  have inOpsemOrder: "respectsCom (actions0 pre) actions (incComAlt ?pre' (incWit ?s')) a"
+    unfolding respectsCom_def
+    proof auto
+      fix b
+      (* TODO: fix opsemOrder *)
+      assume "b \<in> actions0 pre"
+             "(b, a) \<in> incComAlt ?pre' ?wit'"
+      hence ba_in_rel: "(b, a) \<in> incComAlt pre wit"
+        using opsemOrderIsMonotonic downclosed_mo
+        unfolding hbCalcIsMonotonic_def
+        by auto
+      hence "b \<noteq> a"
+        using opsemOrder_isStrictPartialOrder[OF cons]
+        unfolding isStrictPartialOrder_def irrefl_def
+        by auto
+      thus "b \<in> actions"
+        using downclosed' ba_in_rel unfolding downclosed_def by auto
+    next
+      fix b
+      (* TODO: fix opsemOrder *)
+      assume "b \<in> actions0 pre"
+             "b \<in> actions"
+             "(a, b) \<in> incComAlt ?pre' ?wit'"
+      hence ba_in_rel: "(a, b) \<in> incComAlt pre wit"
+        using opsemOrderIsMonotonic downclosed_mo
+        unfolding hbCalcIsMonotonic_def
+        by auto
+      thus False using max `b \<in> actions` by metis 
+    qed
+  have "axsimpConsistentAlt ?pre' ?wit'"
+    using cons downclosed' axsimpConsistent_restriction by metis
+  hence "incStep pre s ?s' a"
+    unfolding incStep_def Let_def 
+    using committed `a \<notin> actions` `a \<in> actions0 pre` witness inOpsemOrder
+    by auto
+  hence "incTrace pre (incInitialState pre) ?s'" using incStep trace by smt
+  thus "\<exists>s'. incTrace pre (incInitialState pre) s' \<and> 
+             incWit s' = incWitRestrict wit ?actions' \<and> 
+             incCommitted s' = ?actions'"
+    by (intro exI[where x="?s'"]) simp
+qed
+
+lemma incConsistentCompleteness:
+  assumes cons: "axsimpConsistent (pre, wit, getRelations pre wit)"
+  shows         "incConsistent (pre, wit, getRelations pre wit)"
+proof -
+  have relOverSb: "relOver (sb pre) (actions0 pre)"
+    using cons by (auto 4 3)
+  have "well_formed_rf (pre, wit, [])" 
+    using cons by auto
+  hence relOverRf: "relOver (rf wit) (actions0 pre)"
+    unfolding well_formed_rf.simps relOver_def 
+    by auto
+  have relOverMo: "relOver (mo wit) (actions0 pre)"
+    using cons by auto
+  have relOverSc: "relOver (sc wit) (actions0 pre)"
+    using cons by auto
+  have relOverLo: "relOver (lo wit) (actions0 pre)"
+    using cons by auto
+  have "tot_empty (pre, wit, [])"
+    using cons by auto
+  hence relOverTot: "relOver (tot wit) (actions0 pre)"
+    unfolding tot_empty.simps by simp
+  have wit_restrict: "incWitRestrict wit (actions0 pre) = wit" 
+    using relOverRf relOverMo relOverSc relOverLo relOverTot
+    unfolding incWitRestrict_def 
+    by (simp add: relRestrict_id)
+  have "relOver (getHb pre wit) (actions0 pre)" 
+    using relOverSb hbRelOver by auto
+  hence relOverHbMinus: "relOver (hbMinusAlt pre wit) (actions0 pre)"
+    unfolding hbMinus.simps 
+              relOver_def 
+              getRelations_simp
+    by auto
+  have downclosed: "downclosed (actions0 pre) (incComAlt pre wit)" 
+    unfolding incComAlt_def
+    using relOverRf relOverMo relOverHbMinus
+    by (simp add: downclosed_relOver)
+  have finite: "finite (actions0 pre)"
+    using cons by auto
+  obtain s where "incTrace pre (incInitialState pre) s"
+                           "incWit s = incWitRestrict wit (actions0 pre)"
+                           "incCommitted s = (actions0 pre)"
+    using existenceIncTrace[OF cons finite _ downclosed]
+    by auto
+  thus ?thesis
+    unfolding incConsistent.simps using wit_restrict by auto
 qed
 
 
 
-(* The incremental model ----------------------------------------------- *)
+section {* The monadic model *}
+
+definition monInvariant :: "pre_execution \<Rightarrow> incState \<Rightarrow> bool" where
+  "monInvariant pre s \<equiv> 
+        axsimpConsistentAlt (preRestrict pre (incCommitted s)) (incWit s)
+      \<and> well_formed_threads_opsem (pre, empty_witness, [])
+      \<and> incCommitted s \<subseteq> actions0 pre"
+
+lemma monInvariantE [elim]:
+  assumes "monInvariant pre s"
+  obtains "axsimpConsistentAlt (preRestrict pre (incCommitted s)) (incWit s)"
+      and "well_formed_threads_opsem (pre, empty_witness, [])"
+      and "incCommitted s \<subseteq> actions0 pre"
+using assms
+unfolding monInvariant_def
+by simp
+
+lemma monInvariantE_incCommittedFinite [elim]:
+  assumes "monInvariant pre s"
+  obtains "finite (incCommitted s)"
+proof -
+  have "incCommitted s \<subseteq> actions0 pre" "finite (actions0 pre)"
+    using assms by auto
+  thus ?thesis using that finite_subset by auto
+qed
+
+subsection {* Elims of auxiliaries *}
+
+lemma sameLocWritesE [elim]:
+  assumes "x \<in> sameLocWrites actions a"
+  obtains "x \<in> actions" "is_write x" "loc_of x = loc_of a"
+using assms
+unfolding sameLocWrites_def
+by auto
+
+lemma sameLocWrites_finite:
+  assumes "finite actions"
+  obtains "finite (sameLocWrites actions a)"
+using assms
+unfolding sameLocWrites_def
+by auto
+
+lemma sameLocLocksUnlocksE [elim]:
+  assumes "x \<in> sameLocLocksUnlocks actions a"
+  obtains "x \<in> actions" "is_lock x \<or> is_unlock x" "loc_of x = loc_of a"
+using assms
+unfolding sameLocLocksUnlocks_def
+by auto
+
+lemma scActionsE [elim]:
+  assumes "x \<in> scActions actions"
+  obtains "x \<in> actions" "is_seq_cst x"
+using assms
+unfolding scActions_def
+by auto
+
+subsection {* Elims of relation constructions *}
+
+lemma monAddToMoE [elim?]:
+  assumes step: "rel [\<in>] monAddToMo pre a s"
+      and inv:  "monInvariant pre s"
+  obtains "rel = mo (incWit s) \<union> (\<lambda>b. (b, a)) ` sameLocWrites (incCommitted s) a"
+using assms
+unfolding monAddToMo_def Let_def
+by auto
+
+lemma auxAddPairToRfE [elim]: 
+  assumes step: "(rel', v) [\<in>] auxAddPairToRf rel w r eq"
+  obtains v_w v_r where "rel' = insert (w, r) rel"
+                        "v = Some (v_w, v_r)"
+                        "value_written_by w = Some v_w"
+                        "value_read_by r = Some v_r"
+                        "eq v_w v_r"
+using assms
+unfolding auxAddPairToRf_def
+apply (cases "value_written_by w", auto)
+by (cases "value_read_by r", auto)
+
+lemma auxAddToRfLoadE [elim?]:
+  assumes step: "(rel, v) [\<in>] auxAddToRfLoad pre a s eq"
+      and inv:  "monInvariant pre s"
+  obtains w where "w \<in> sameLocWrites (incCommitted s) a" 
+                  "(rel, v) [\<in>] auxAddPairToRf (rf (incWit s)) w a eq"
+        | "rel = rf (incWit s)"
+proof (cases "rel = rf (incWit s)")
+  case True
+  thus ?thesis using that by metis
+next
+  case False
+  have "finite (sameLocWrites (incCommitted s) a)"
+    using inv sameLocWrites_finite by auto
+  then obtain w where w: "w \<in> sameLocWrites (incCommitted s) a"
+                         "(rel, v) [\<in>] auxAddPairToRf (rf (incWit s)) w a eq"
+    using step False
+    unfolding auxAddToRfLoad_def
+    by auto
+  thus ?thesis using w that by auto
+qed
+
+lemma monAddToRfLoadE [elim?]:
+  assumes step: "rel [\<in>] monAddToRfLoad pre a s"
+      and inv:  "monInvariant pre s"
+  obtains w v where "w \<in> sameLocWrites (incCommitted s) a" 
+                    "(rel, v) [\<in>] auxAddPairToRf (rf (incWit s)) w a op ="
+        | "rel = rf (incWit s)"
+proof -
+  obtain v where v: "(rel, v) [\<in>] auxAddToRfLoad pre a s op ="
+    using step
+    unfolding monAddToRfLoad_def
+    by auto
+  thus ?thesis
+    using that auxAddToRfLoadE[OF v inv]
+    by (cases "rel = rf (incWit s)") metis+
+qed
+
+lemma auxAddToRfRmwE [elim?]:
+  assumes step: "(rel, v) [\<in>] auxAddToRfRmw pre a s eq"
+      and inv:  "monInvariant pre s"
+  obtains w where "w \<in> sameLocWrites (incCommitted s) a"
+                  "\<forall>w' \<in> sameLocWrites (incCommitted s) a. (w, w') \<notin> mo (incWit s)"
+                  "(rel, v) [\<in>] auxAddPairToRf (rf (incWit s)) w a eq"
+        | "sameLocWrites (incCommitted s) a = {}"
+          "rel = rf (incWit s)"
+proof (cases "sameLocWrites (incCommitted s) a = {}")
+  case True
+  thus ?thesis 
+    using step that unfolding auxAddToRfRmw_def by auto
+next
+  case False
+  have "finite (sameLocWrites (incCommitted s) a)"
+    using inv sameLocWrites_finite by auto
+  then obtain w where w: "w \<in> sameLocWrites (incCommitted s) a"
+                         "\<forall>w' \<in> sameLocWrites (incCommitted s) a. (w, w') \<notin> mo (incWit s)"
+                         "(rel, v) [\<in>] auxAddPairToRf (rf (incWit s)) w a eq"
+    using step False
+    unfolding auxAddToRfRmw_def Let_def
+    by auto
+  thus ?thesis using w that by auto
+qed
+
+lemma monAddToRfRmwE [elim?]:
+  assumes step: "rel [\<in>] monAddToRfRmw pre a s"
+      and inv:  "monInvariant pre s"
+  obtains w v where "w \<in> sameLocWrites (incCommitted s) a" 
+                    "\<forall>w' \<in> sameLocWrites (incCommitted s) a. (w, w') \<notin> mo (incWit s)"
+                    "(rel, v) [\<in>] auxAddPairToRf (rf (incWit s)) w a op ="
+        | "sameLocWrites (incCommitted s) a = {}"
+          "rel = rf (incWit s)"
+proof -
+  obtain v where v: "(rel, v) [\<in>] auxAddToRfRmw pre a s op ="
+    using step
+    unfolding monAddToRfRmw_def
+    by auto
+  thus ?thesis
+    using that auxAddToRfRmwE[OF v inv]
+    by (cases "rel = rf (incWit s)") metis+
+qed
+
+subsection {* Elims of monStep *}
+
+lemma monStepE_action [elim]:
+  assumes monStep:  "(a, s2) [\<in>] monStep pre s1"
+      and inv:  "monInvariant pre s"
+  obtains "a \<in> actions0 pre" "a \<notin> incCommitted s1"
+proof -
+  have "finite (actions0 pre)"
+    using inv by auto
+  hence "a \<in> actions0 pre" "a \<notin> incCommitted s1"
+    using monStep
+    unfolding monStep_def Let_def
+    by auto
+  thus ?thesis using that by simp
+qed
+
+lemma monStepE_committed [elim]:
+  assumes monStep:  "(a, s2) [\<in>] monStep pre s1"
+  obtains "incCommitted s2 = insert a (incCommitted s1)"
+using monStep
+unfolding monStep_def Let_def
+by auto
+
+lemmas monPerformActions_def = 
+  monPerformLock_def
+  monPerformUnlock_def
+  monPerformLoad_def
+  monPerformStore_def
+  monPerformRmw_def
+  monPerformFence_def
+  monPerformBlocked_rmw_def
+
+lemma monStepE_rf [elim?, consumes 1]:
+  assumes monStep: "(a, s2) [\<in>] monStep pre s1"
+  obtains (load)   "is_load a" "rf (incWit s2) [\<in>] monAddToRfLoad pre a s1"
+        | (rmw)    "is_RMW a" "rf (incWit s2) [\<in>] monAddToRfRmw pre a s1"
+        | (other)  "\<not>is_read a" "rf (incWit s2) = rf (incWit s1)"
+using assms
+unfolding monStep_def monPerformActions_def Let_def
+by (cases a) auto
+
+lemma monStepE_rf2 [elim?]:
+  assumes monStep: "(a, s2) [\<in>] monStep pre s1"
+      and inv:     "monInvariant pre s1"
+  obtains w where "rf (incWit s2) = insert (w, a) (rf (incWit s1))"
+                  "w \<in> sameLocWrites (incCommitted s1) a"
+        | "rf (incWit s2) = rf (incWit s1)"
+proof (cases rule: monStepE_rf[OF monStep])
+  case 1
+  thus ?thesis
+    using that
+    by (cases rule: monAddToRfLoadE[OF 1(2) inv]) auto
+next
+  case 2
+  thus ?thesis
+    using that
+    by (cases rule: monAddToRfRmwE[OF 2(2) inv]) auto
+next
+  case 3
+  thus ?thesis using that by auto
+qed
+
+lemma monStepE_mo [elim?]:
+  assumes monStep: "(a, s2) [\<in>] monStep pre s1"
+      and inv:     "monInvariant pre s1"
+  obtains (store) "is_write a" 
+                  "is_at_atomic_location (lk pre) a"
+                  "mo (incWit s2) [\<in>] monAddToMo pre a s1"
+        | (other) "\<not>is_RMW a"
+                  "\<not>(is_store a \<and> is_at_atomic_location (lk pre) a)" 
+                  "mo (incWit s2) = mo (incWit s1)"
+proof (cases "is_write a \<and> is_at_atomic_location (lk pre) a")
+  assume a: "is_write a \<and> is_at_atomic_location (lk pre) a"
+  hence "mo (incWit s2) [\<in>] monAddToMo pre a s1"
+    using monStep
+    unfolding monStep_def monPerformActions_def Let_def
+    by (cases a) auto
+  thus ?thesis using a store by auto
+next
+  assume a: "\<not>(is_write a \<and> is_at_atomic_location (lk pre) a)"
+  hence a2: "\<not>(is_store a \<and> is_at_atomic_location (lk pre) a)" 
+    by (cases a) auto
+  have "a \<in> actions0 pre"
+    using monStep inv by auto
+  have "actions_respect_location_kinds (actions0 pre) (lk pre)"
+    using inv by auto
+  hence "is_RMW a \<Longrightarrow> is_at_atomic_location (lk pre) a"
+    using is_RMWE_location_kind[OF _ `a \<in> actions0 pre`]
+    by auto
+  hence a3: "\<not>is_RMW a" using a  `a \<in> actions0 pre` by auto
+  hence "mo (incWit s2) = mo (incWit s1)"
+    using a monStep
+    unfolding monStep_def monPerformActions_def Let_def
+    by (cases a) auto
+  thus ?thesis using a2 a3 other by auto
+qed
+
+lemma monStepE_mo2 [elim?]:
+  assumes monStep: "(a, s2) [\<in>] monStep pre s1"
+      and inv:     "monInvariant pre s1"
+  obtains (store) "is_write a" 
+                  "is_at_atomic_location (lk pre) a"
+                  "mo (incWit s2) =    mo (incWit s1)
+                                    \<union> (\<lambda>b. (b, a)) ` sameLocWrites (incCommitted s1) a"
+        | (other) "\<not>is_RMW a"
+                  "\<not>(is_store a \<and> is_at_atomic_location (lk pre) a)" 
+                  "mo (incWit s2) = mo (incWit s1)"
+proof (cases rule: monStepE_mo[OF monStep inv])
+  case 1
+  thus ?thesis
+    using monAddToMoE[OF _ inv] using that by metis
+next
+  case 2
+  thus ?thesis using that by auto
+qed
+
+lemma monStepE_mo3 [elim?]:
+  assumes monStep: "(a, s2) [\<in>] monStep pre s1"
+      and inv:     "monInvariant pre s1"
+  obtains "mo (incWit s1) = relRestrict (mo (incWit s2)) (incCommitted s1)"
+proof -
+  have cons_mo: "consistent_mo (preRestrict pre (incCommitted s1), incWit s1, [])"
+    using inv by auto
+  hence s1: "mo (incWit s1) = relRestrict (mo (incWit s1)) (incCommitted s1)"
+    unfolding relRestrict_def by auto 
+  show ?thesis
+    proof (cases rule: monStepE_mo2[OF monStep inv])
+      case 1
+      have "a \<notin> incCommitted s1" using monStep inv by auto
+      hence "  relRestrict (mo (incWit s2)) (incCommitted s1)
+             = relRestrict (mo (incWit s1)) (incCommitted s1)"
+        using 1 by auto
+      thus ?thesis using 1 s1 that by auto
+    next
+      case 2
+      thus ?thesis using 2 s1 that by auto
+    qed
+qed
+
+lemma monStepE_lo [elim?]:
+  assumes monStep: "(a, s2) [\<in>] monStep pre s1"
+  obtains (lock)  "is_lock a \<or> is_unlock a" 
+                  "lo (incWit s2) [\<in>] monAddToLo pre a s1"
+        | (other) "\<not>is_lock a" 
+                  "\<not>is_unlock a" 
+                  "lo (incWit s2) = lo (incWit s1)"
+using assms
+unfolding monStep_def monPerformActions_def Let_def
+by (cases a) auto
+
+lemma monStepE_sc [elim?]:
+  assumes monStep: "(a, s2) [\<in>] monStep pre s1"
+  obtains (sc)    "is_seq_cst a" 
+                  "sc (incWit s2) [\<in>] monAddToSc pre a s1"
+        | (other) "\<not>is_seq_cst a" 
+                  "sc (incWit s2) = sc (incWit s1)"
+using assms
+unfolding monStep_def monPerformActions_def Let_def 
+apply (cases a, auto)
+by (cases "is_seq_cst a", auto)+
+
+lemma monStepE_tot [elim?]:
+  assumes monStep: "(a, s2) [\<in>] monStep pre s1"
+  obtains "tot (incWit s2) = tot (incWit s1)"
+unfolding incToEx_def Let_def tot_empty.simps
+using monStep
+unfolding monStep_def monPerformActions_def Let_def
+by (cases a) auto
+
+subsection {* Simps of checkXxx predicates *}
+
+lemma monCheckConsistency_simp [simp]:
+  shows "  x [\<in>] monCheckConsistency (pre, wit, getRelations pre wit)
+         = axsimpConsistentAlt pre wit"
+unfolding monCheckConsistency_def
+by simp
+
+lemma monCheckWitRestrict_simp [simp]:
+  shows "  x [\<in>] monCheckWitRestrict wit1 committed wit2
+         = (incWitRestrict wit1 committed = wit2)"
+unfolding monCheckWitRestrict_def
+by simp
+
+lemma monCheckCommitmentOrder_simp [simp]:
+  shows "  x [\<in>] monCheckCommitmentOrder actions (pre, wit, getRelations pre wit) committed a
+         = (respectsCom actions committed (incComAlt pre wit) a)"
+unfolding monCheckCommitmentOrder.simps Let_def
+by simp
+
+subsection {* Soundness *}
+
+(* assumptions *)
+
+lemma monStep_assumptions:
+  assumes monStep: "(a, s2) [\<in>] monStep pre s1"
+      and inv:     "monInvariant pre s1"
+  shows   "assumptions (incToEx pre s2)" 
+unfolding incToEx_def Let_def assumptions.simps
+proof auto
+  have rf: "finite_prefixes (rf (incWit s1)) (actions0 (preRestrict pre (incCommitted s1)))"
+    using inv by blast
+  show "finite_prefixes (rf (incWit s2)) (actions0 pre \<inter> incCommitted s2)"
+    proof (cases rule: monStepE_rf2[OF monStep inv])
+      case 1
+      show ?thesis sorry
+    next
+      case 2
+      show ?thesis sorry
+    qed
+oops
+
+(* tot_empty *)
+
+lemma monStep_tot_empty:
+  assumes monStep: "(a, s2) [\<in>] monStep pre s1"
+      and inv:     "monInvariant pre s1"
+  shows   "tot_empty (incToEx pre s2)"
+proof -
+  have "tot (incWit s1) = {}"
+    using inv by auto
+  thus ?thesis
+    using monStepE_tot[OF monStep]
+    unfolding tot_empty.simps Let_def incToEx_def
+    by auto
+qed
+
+(* well_formed_threads_opsem *)
+
+lemma monStep_well_formed_threads_opsem:
+  assumes monStep: "(a, s2) [\<in>] monStep pre s1"
+      and inv:     "monInvariant pre s1"
+  shows   "well_formed_threads_opsem (incToEx pre s2)"
+proof -
+  have "well_formed_threads_opsem (pre, empty_witness, [])"
+    using inv by auto
+  hence "well_formed_threads_opsem (preRestrict pre (incCommitted s2), empty_witness, [])"
+    using well_formed_threads_opsem_restriction by auto
+  thus ?thesis
+    unfolding incToEx_def Let_def
+    by (cases "incWit s2 = empty_witness") auto
+qed
+
+(* well_formed_rf *)
+
+lemma monStep_well_formed_rf_aux:
+  assumes monStep: "(a, s2) [\<in>] monStep pre s1"
+      and inv:     "monInvariant pre s1"
+      and rf:      "rf (incWit s2) = rf (incWit s1)"
+  shows   "well_formed_rf (incToEx pre s2)"
+proof -
+  have cons_rf: "well_formed_rf (preRestrict pre (incCommitted s1), incWit s1, [])"
+    using inv unfolding incToEx_def Let_def by auto
+  have com: "incCommitted s2 = insert a (incCommitted s1)"
+    using monStep by auto
+  show ?thesis
+    unfolding incToEx_def Let_def well_formed_rf.simps 
+    unfolding com rf
+    using cons_rf
+    by auto
+qed
+
+lemma well_formed_rfIE:
+  assumes cons_rf:  "well_formed_rf (pre, wit, rel)"
+      and rf:       "rf wit' = insert (w, r) (rf wit)"
+      and actions:  "actions0 pre' \<supseteq> actions0 pre"
+      and r_and_w:  "w \<in> actions0 pre'"
+                    "r \<in> actions0 pre'"
+                    "loc_of w = loc_of r"
+                    "is_write w"
+                    "is_read r"
+                    "value_read_by r = value_written_by w"
+      and r_is_new: "r \<notin> actions0 pre"
+  shows   "well_formed_rf (pre', wit', rel')"
+unfolding well_formed_rf.simps 
+proof auto
+  fix a b
+  assume in_rf: "(a, b) \<in> rf wit'"
+  thus "a \<in> actions0 pre'"
+       "b \<in> actions0 pre'"
+       "loc_of a = loc_of b"
+       "is_write a"
+       "is_read b"
+       "value_read_by b = value_written_by a"
+    unfolding rf using cons_rf r_and_w actions by auto
+  fix a'
+  assume in_rf': "(a', b) \<in> rf wit'"
+  thus "a = a'"
+    proof (cases "b = r")
+      case True
+      have "(a, r) \<notin> rf wit" "(a', r) \<notin> rf wit"
+        using cons_rf r_is_new by auto
+      hence "a = w" "a' = w"
+        using in_rf in_rf' True unfolding rf by auto
+      thus ?thesis by auto
+    next
+      case False
+      hence "(a, b) \<in> rf wit" "(a', b) \<in> rf wit"
+        using in_rf in_rf' unfolding rf by auto
+      thus "a = a'"
+        using cons_rf by auto
+    qed
+qed
+
+lemma monStep_well_formed_rf:
+  assumes monStep: "(a, s2) [\<in>] monStep pre s1"
+      and inv:     "monInvariant pre s1"
+  shows   "well_formed_rf (incToEx pre s2)"
+proof -
+  have cons_rf: "well_formed_rf (preRestrict pre (incCommitted s1), incWit s1, [])"
+    using inv unfolding incToEx_def Let_def by auto
+  have com: "incCommitted s2 = insert a (incCommitted s1)"
+    using monStep by auto
+  have a: "a \<in> incCommitted s2" "a \<in> actions0 pre" "a \<notin> incCommitted s1"
+    using monStep inv by auto
+  show ?thesis
+    proof (cases rule: monStepE_rf[OF monStep])
+      case 1 (* load *)
+      hence "is_read a" by (intro is_readI) auto
+      show ?thesis
+        proof (cases rule: monAddToRfLoadE[OF 1(2) inv])
+          case (1 w) 
+          hence wit: "rf (incWit s2) = insert (w, a) (rf (incWit s1))"
+            by auto
+          show ?thesis
+            using cons_rf
+            unfolding incToEx_def Let_def 
+            apply (elim well_formed_rfIE[OF _ wit])
+            using 1 com inv a `is_read a`
+            by auto          
+        next
+          case 2 (* rf (incWit s2) = rf (incWit s1) *)
+          thus ?thesis
+            using monStep_well_formed_rf_aux monStep inv
+            by metis
+        qed
+    next
+      case 2 (* rmw *)
+      hence "is_read a" by auto
+      show ?thesis
+        proof (cases rule: monAddToRfRmwE[OF 2(2) inv])
+          case (1 w)
+          hence wit: "rf (incWit s2) = insert (w, a) (rf (incWit s1))"
+            by auto
+          show ?thesis
+            using cons_rf
+            unfolding incToEx_def Let_def 
+            apply (elim well_formed_rfIE[OF _ wit])
+            (* assumption 1(2) criples auto, so we don't add it. *)
+            using 1(1) 1(3) com inv a `is_read a`
+            by auto
+        next
+          case 2 (* rf (incWit s2) = rf (incWit s1) *)
+          thus ?thesis
+            using monStep_well_formed_rf_aux monStep inv
+            by metis
+        qed
+    next
+      case 3 (* other *)
+      thus ?thesis
+        using monStep_well_formed_rf_aux monStep inv
+        by metis
+    qed
+qed
+
+(* locks_only_consistent_locks *)
+
+(* locks_only_consistent_lo *)
+
+(* consistent_mo *)
+
+(* sc_accesses_consistent_sc *)
+
+(* sc_fenced_sc_fences_heeded *)
+
+(* consistent_hb *)
+
+(* det_read_alt *)
+
+(* consistent_non_atomic_rf *)
+
+(* consistent_atomic_rf *)
+
+(* coherent_memory_use *)
+
+(* rmw_atomicity *)
+
+lemma monStep_rmw_atomicity:
+  assumes monStep: "(a, s2) [\<in>] monStep pre s1"
+      and inv:     "monInvariant pre s1"
+  shows   "rmw_atomicity (incToEx pre s2)"
+unfolding incToEx_def Let_def
+unfolding rmw_atomicity.simps
+proof clarsimp
+  have cons_rf: "well_formed_rf (preRestrict pre (incCommitted s1), incWit s1, [])"
+    using inv by auto
+  have cons_mo: "consistent_mo (preRestrict pre (incCommitted s1), incWit s1, [])"
+    using inv by auto
+  have cons_rmw: "rmw_atomicity (preRestrict pre (incCommitted s1), incWit s1, [])"
+    using inv by auto
+  have com: "incCommitted s2 = insert a (incCommitted s1)"
+    using monStep by auto
+  fix w r
+  assume w: "w \<in> actions0 pre" "w \<in> incCommitted s2"
+     and r: "r \<in> actions0 pre" "r \<in> incCommitted s2" "is_RMW r"
+  have a: "a \<notin> incCommitted s1" "a \<in> actions0 pre"
+    using monStep inv by auto
+  hence "(a, r) \<notin> rf (incWit s1)"
+    using cons_rf by auto
+  hence "(a, r) \<notin> rf (incWit s2)"
+    using a
+    by (cases rule: monStepE_rf2[OF monStep inv]) auto
+  have "(a, r) \<notin> mo (incWit s1)"
+    using a cons_mo by auto
+  hence "(a, r) \<notin> mo (incWit s2)"
+    using a
+    by (cases rule: monStepE_mo2[OF monStep inv]) auto
+  have "(w, a) \<notin> rf (incWit s1)"
+    using a cons_rf by auto
+  show "adjacent_less_than (mo (incWit s2)) (actions0 pre \<inter> incCommitted s2) w r 
+        = ((w, r) \<in> rf (incWit s2))"
+    proof (cases "w = a")
+      assume "w = a"
+      have "\<not>adjacent_less_than (mo (incWit s2)) (actions0 pre \<inter> incCommitted s2) a r "
+        using `(a, r) \<notin> mo (incWit s2)` by auto
+      thus ?thesis
+        using `(a, r) \<notin> rf (incWit s2)` `w = a` by auto
+    next
+      assume "w \<noteq> a"
+      hence w2: "w \<in> incCommitted s1"
+        using w monStep by auto
+      show ?thesis
+        proof (cases "r = a")
+          assume "r \<noteq> a"
+          hence r2: "r \<in> incCommitted s1"
+            using r monStep by auto
+          have mo_eq: "((w, r) \<in> mo (incWit s1)) = ((w, r) \<in> mo (incWit s2))"
+            using w w2 r r2 by (cases rule: monStepE_mo3[OF monStep inv]) auto       
+          have "  (\<exists>z\<in>actions0 pre \<inter> incCommitted s2. 
+                       (w, z) \<in> mo (incWit s2) \<and> (z, r) \<in> mo (incWit s2))
+                 = (\<exists>z\<in>actions0 pre \<inter> incCommitted s1. 
+                       (w, z) \<in> mo (incWit s1) \<and> (z, r) \<in> mo (incWit s1))"
+            unfolding com
+            using `(a, r) \<notin> mo (incWit s2)` w2 r2
+            by (cases rule: monStepE_mo3[OF monStep inv]) auto
+          hence "  adjacent_less_than (mo (incWit s2)) (actions0 pre \<inter> incCommitted s2) w r
+                = adjacent_less_than (mo (incWit s1)) (actions0 pre \<inter> incCommitted s1) w r"
+            unfolding adjacent_less_than_def using mo_eq by auto
+          also have "... = ((w, r) \<in> rf (incWit s1))"
+            using cons_rmw w w2 r r2 by auto
+          also have "... = ((w, r) \<in> rf (incWit s2))"
+            using `r \<noteq> a`
+            by (cases rule: monStepE_rf2[OF monStep inv]) auto
+          finally show ?thesis .
+        next
+          assume "r = a"
+          hence "is_RMW a" using r by auto
+          hence mo_s2: "  mo (incWit s2)
+                        = mo (incWit s1) \<union> (\<lambda>b. (b, a)) ` sameLocWrites (incCommitted s1) a"
+             by (cases rule: monStepE_mo2[OF monStep inv]) auto
+          have rmw_step: "rf (incWit s2) [\<in>] monAddToRfRmw pre a s1"
+            using `is_RMW a`
+            by (cases rule: monStepE_rf[OF monStep], cases a) auto
+          show ?thesis
+            proof (cases "w \<in> sameLocWrites (incCommitted s1) a")
+              assume w_not_same_loc: "w \<notin> sameLocWrites (incCommitted s1) a"
+              hence "(w, a) \<notin> rf (incWit s2)"
+                using `(w, a) \<notin> rf (incWit s1)` 
+                by (cases rule: monAddToRfRmwE[OF rmw_step inv]) auto
+              have "(w, a) \<notin> mo (incWit s1)"
+                using a cons_mo by auto
+              hence "(w, a) \<notin> mo (incWit s2)"
+                 using w_not_same_loc mo_s2 by auto
+              hence "\<not> adjacent_less_than (mo (incWit s2)) (actions0 pre \<inter> incCommitted s2) w a"
+                 by auto                 
+              thus ?thesis 
+                using `r = a` `(w, a) \<notin> rf (incWit s2)` by auto
+            next
+              assume w_same_loc: "w \<in> sameLocWrites (incCommitted s1) a"
+              then obtain w' where w':     "w' \<in> sameLocWrites (incCommitted s1) a"
+                               and w'_max: "\<forall>w''\<in>sameLocWrites (incCommitted s1) a. 
+                                                  (w', w'') \<notin> mo (incWit s1)"
+                               and rf_s2:  "rf (incWit s2) = insert (w', a) (rf (incWit s1))"
+                by (cases rule: monAddToRfRmwE[OF rmw_step inv]) auto
+              have w'_a_in_mo: "(w', a) \<in> mo (incWit s2)"
+                using w' mo_s2 by auto
+              show ?thesis
+                proof (cases "w = w'")
+                  assume "w = w'"
+                  have "adjacent_less_than (mo (incWit s2)) (actions0 pre \<inter> incCommitted s2) w' a"
+                    unfolding adjacent_less_than_def
+                    using w'_a_in_mo
+                    proof auto
+                      fix z
+                      assume "(z, a) \<in> mo (incWit s2)"
+                      moreover have "(z, a) \<notin> mo (incWit s1)"
+                        using a cons_mo by auto
+                      ultimately have "z \<in> sameLocWrites (incCommitted s1) a"
+                        using mo_s2 by auto
+                      hence "(w', z) \<notin> mo (incWit s1)" "z \<noteq> a"
+                        using w'_max a by auto
+                      hence "(w', z) \<notin> mo (incWit s2)"
+                        using mo_s2 by auto
+                      moreover assume "(w', z) \<in> mo (incWit s2)"
+                      ultimately show False by simp
+                    qed
+                  thus ?thesis using rf_s2 `r = a` `w = w'` by auto
+                next
+                  assume "w \<noteq> w'"
+                  hence "(w, a) \<notin> rf (incWit s2)"
+                    using rf_s2 `(w, a) \<notin> rf (incWit s1)` by auto
+                  have w'2: "w' \<in> actions0 pre" 
+                            "w' \<in> incCommitted s1"
+                            "is_write w'"
+                            "loc_of w' = loc_of a"
+                    using w' inv by auto
+                  have w2: "w \<in> actions0 pre" 
+                           "w \<in> incCommitted s1"
+                           "is_write w"
+                           "loc_of w = loc_of a"
+                    using w_same_loc inv by auto
+                  have "is_at_atomic_location (lk pre) a"
+                    using is_RMWE_location_kind[OF `is_RMW a` ]
+                    using inv a
+                    by auto
+                  hence "is_at_atomic_location (lk pre) w" 
+                    using w2 same_loc_atomic_location by metis
+                  hence "(w, w') \<in> mo (incWit s1) \<or> (w', w) \<in> mo (incWit s1)"
+                    using cons_mo w2 w'2 `w \<noteq> w'` 
+                    unfolding consistent_mo.simps
+                    by auto
+                  hence "(w, w') \<in> mo (incWit s1)" 
+                    using w'_max w_same_loc by auto
+                  hence "(w, w') \<in> mo (incWit s2)" 
+                    using mo_s2 by auto
+                  hence "\<not> adjacent_less_than (mo (incWit s2)) (actions0 pre \<inter> incCommitted s2) w a"
+                     unfolding adjacent_less_than_def
+                     using w'_a_in_mo w'2 com
+                     by auto
+                  thus ?thesis using `(w, a) \<notin> rf (incWit s2)` `r = a` by auto
+                qed
+            qed
+        qed
+    qed
+qed
+
+(* sc_accesses_sc_reads_restricted *)
+
+(* Invariant *)
+
+lemma monStepInvariant:
+  assumes monStep: "(a, s2) [\<in>] monStep pre s1"
+      and inv:     "monInvariant pre s1"
+  shows   "monInvariant pre s2"
+proof -
+  have "finite (actions0 pre)"
+    using inv by auto
+  thus ?thesis
+    using monStep inv
+    unfolding monInvariant_def
+    unfolding monStep_def Let_def
+    apply auto sorry (* Not true yet *)
+qed
+
+lemma monStepSoundness:
+  assumes monStep: "(a, s2) [\<in>] monStep pre s1"
+      and inv:     "monInvariant pre s1"
+  shows   "incStep pre s1 s2 a"
+using monStep inv
+using monStepInvariant[OF monStep inv]
+unfolding monInvariant_def
+          monStep_def Let_def incStep_def
+by auto
+
+subsection {* Completeness *}
+
+(* modification order *)
+
+lemma step_mo_not_atomic_write:
+  assumes cons:      "axsimpConsistentAlt pre' wit'"
+      and committed: "actions0 pre' = insert a committed"
+      and a:         "is_at_non_atomic_location (lk pre') a \<or> \<not> is_write a"
+  shows              "mo wit' = mo (incWitRestrict wit' committed)"
+proof auto
+  fix b c
+  assume in_mo: "(b, c) \<in> mo wit'"
+  hence b: "b \<in> actions0 pre' \<and> is_at_atomic_location (lk pre') b \<and> is_write b" 
+    and c: "c \<in> actions0 pre' \<and> is_at_atomic_location (lk pre') c \<and> is_write c"
+    using cons by auto
+  hence "a \<noteq> b" "a \<noteq> c" using a by auto
+  thus "b \<in> committed" "c \<in> committed" 
+    using b c committed by auto
+qed
+
+(*
+lemma step_mo_atomic_write:
+  assumes cons1:     "axsimpConsistentAlt pre  wit"
+      and cons2:     "axsimpConsistentAlt pre' wit'"
+      and wit:       "wit = incWitRestrict wit' (actions0 pre)"
+      and committed: "actions0 pre' = insert a (actions0 pre)"
+      and a:         "  is_at_atomic_location (lk pre') a \<and> is_write a 
+                      \<and> a \<in> actions0 pre \<and> a \<notin> incCommitted s"
+  shows   "mo wit' [\<in>] monAddToMo pre a s"
+unfolding monAddToMo_def Let_def
+proof simp
+  let ?succ     = "(\<lambda>b. (b, a)) ` {x \<in> actions0 pre. x \<in> incCommitted s \<and> x \<noteq> a \<and> is_write x \<and> loc_of x = loc_of a}"
+  let ?new_mo   = "mo (incWit s) \<union> ?succ"
+  show "mo (incWit s')  = ?new_mo"
+    proof (intro equalityI subsetI)
+      fix x
+      assume "x \<in> mo (incWit s')"
+      then obtain b c where "(b, c) = x" "(b, c) \<in> mo (incWit s')" by (cases x) fast
+      have "(b, c) \<in> ?new_mo"
+        proof (cases "b = a")
+        next
+          assume "b = a"
+          have not_in_mo_bc: "(b, c) \<notin> mo (incWit s)" using a wit `b = a` by auto
+          have "(c, b) \<notin> mo (incWit s')" 
+            using consistent_mo_aux2[OF cons2 `(b, c) \<in> mo (incWit s')`] by simp
+          hence not_in_mo_cb: "(c, b) \<notin> mo (incWit s)" using wit by auto 
+          have "c \<notin> incCommitted s"
+            proof
+              assume "c \<in> incCommitted s"
+              have "b \<in> actions0 pre \<and> c \<in> actions0 pre \<and> b \<noteq> c \<and> 
+                    is_write b \<and> is_write c \<and> loc_of b = loc_of c \<and> 
+                    is_at_atomic_location (lk pre) b"
+                using consistent_mo_aux2[OF cons2 `(b, c) \<in> mo (incWit s')`] incCommitted
+                by auto
+              hence "(b, c) \<in> mo (incWit s) \<or> (c, b) \<in> mo (incWit s)"
+                using `c \<in> incCommitted s` consistent_mo_aux1[OF cons1] by auto
+              thus False using not_in_mo_bc not_in_mo_cb by simp
+              qed
+          hence "(b, c) \<in> ?succ"
+            using `b = a` consistent_mo_aux2[OF cons2 `(b, c) \<in> mo (incWit s')`] by auto
+          thus "(b, c) \<in> ?new_mo" by simp
+        next
+          assume "b \<noteq> a"
+          hence "b \<in> incCommitted s" 
+            using consistent_mo_aux2[OF cons2 `(b, c) \<in> mo (incWit s')`] incCommitted by auto  
+          hence "(b, c) \<in> mo (incWit s)"
+            using wit `(b, c) \<in> mo (incWit s')` by auto
+          thus "(b, c) \<in> ?new_mo" by simp
+        qed
+      thus "x \<in> ?new_mo" using `(b, c) = x` by simp
+    next
+      fix x
+      assume "x \<in> ?new_mo"
+      show "x \<in> mo (incWit s')"
+        using `x \<in> ?new_mo`
+        proof (elim UnE)
+          assume "x \<in> mo (incWit s)" 
+          thus "x \<in> mo (incWit s')" using wit by auto
+        next
+          assume "x \<in> ?succ"
+          then obtain b c where "(b, c) = x" "(b, c) \<in> ?succ" by (cases x) fast
+          hence "(c, b) \<notin> mo (incWit s')" using consistent_mo_aux2[OF cons2] incCommitted by fast
+          hence "(b, c) \<in> mo (incWit s')"
+            using `(b, c) \<in> ?succ` a cons2 incCommitted 
+            using consistent_mo_aux1[where a=a and b=c and wit="incWit s'"] 
+            by auto
+          thus "x \<in> mo (incWit s')" using `(b, c) = x` by simp
+        qed
+    qed
+qed
+*)
+
+
 
 end
